WP1-Programming-Languages-Semantics/WP11-C-semantics/src/IMP-Lenses/utp/utp_rel.thy
@@ -5,8 +5,8 @@ text{*Instead of using a deep-embedding for the abstract syntax we use shallow e
       We use abbreviation in order that we do not hide the core theory behind
       another definition layer. Which makes it more suited for exploitation by simp, auto, etc*}
 
-theory Commands 
-imports "utp/utp_designs"
+theory utp_rel 
+imports "utp_pred" "utp_alphabet" "utp_urel_setup"
 
 begin
 
@@ -19,13 +19,27 @@ translations
   (type) "('\<alpha>, '\<beta>) rel" <= (type) "('\<alpha> \<times> '\<beta>) upred"
 
 subsection{*SKIP*}
+
+
+definition skip_ra :: "('\<beta>, '\<alpha>) lens \<Rightarrow>'\<alpha> hrel" where
+[urel_defs]: "skip_ra v = ($v\<acute> =\<^sub>u $v)"
+
+syntax
+  "_skip_ra" :: "salpha \<Rightarrow> logic" ("II\<^bsub>_\<^esub>")
+
+translations
+  "_skip_ra v" == "CONST skip_ra v"
+
 lift_definition assigns_r :: "'\<alpha> usubst \<Rightarrow> '\<alpha> hrel" ("\<langle>_\<rangle>\<^sub>a")
   is "\<lambda> \<sigma> (A, A'). A' = \<sigma>(A)" .
 
-definition skip_r :: "'\<alpha> hrel"("SKIP") where
+definition skip_r :: "'\<alpha> hrel" where
 [urel_defs]:"skip_r = assigns_r id"
 
 subsection{*Assign*}
+
+definition assigns_ra :: "'\<alpha> usubst \<Rightarrow> ('\<beta>, '\<alpha>) lens \<Rightarrow> '\<alpha> hrel" ("\<langle>_\<rangle>\<^bsub>_\<^esub>") where
+"\<langle>\<sigma>\<rangle>\<^bsub>a\<^esub> = (\<lceil>\<sigma>\<rceil>\<^sub>s \<dagger> II\<^bsub>a\<^esub>)"
 
 abbreviation assign_r :: "('t, '\<alpha>) uvar \<Rightarrow> ('t, '\<alpha>) uexpr \<Rightarrow> '\<alpha> hrel"  where 
   "assign_r v expr \<equiv> assigns_r [v \<mapsto>\<^sub>s expr]"
@@ -36,17 +50,42 @@ abbreviation assign_2_r ::
 
 subsection{*Conditional*}
 
-definition cond::"'\<alpha> upred \<Rightarrow> '\<alpha> upred \<Rightarrow> '\<alpha> upred \<Rightarrow> '\<alpha> upred" ("IF (_)/ THEN (_) ELSE (_)"  70)
-where [urel_defs]:"(IF b THEN P ELSE Q) = ((b \<and> P) \<or> ((\<not> b) \<and> Q))"
-
 abbreviation rcond::"('\<alpha>, '\<beta>) rel \<Rightarrow> '\<alpha> cond \<Rightarrow> ('\<alpha>, '\<beta>) rel \<Rightarrow> ('\<alpha>, '\<beta>) rel"
                                                           ("(3_ \<triangleleft> _ \<triangleright>\<^sub>r/ _)" [52,0,53] 52)
-where "(P \<triangleleft> b \<triangleright>\<^sub>r Q) \<equiv> (IF \<lceil>b\<rceil>\<^sub>< THEN P ELSE Q)"
+where "(P \<triangleleft> b \<triangleright>\<^sub>r Q) \<equiv> (P \<triangleleft>\<lceil>b\<rceil>\<^sub>< \<triangleright> Q)"
 
 subsection{*Sequential composition*}
 
-lift_definition seqr::"('\<alpha>, '\<beta>) rel \<Rightarrow> ('\<beta>, '\<gamma>) rel \<Rightarrow> ('\<alpha>, '\<gamma>) rel" (infixr ";;" 51) is
+lift_definition seqr::"('\<alpha>, '\<beta>) rel \<Rightarrow> ('\<beta>, '\<gamma>) rel \<Rightarrow> ('\<alpha>, '\<gamma>) rel"  is
   "\<lambda> P Q r. r \<in> ({p. P p} O {q. Q q})" .
+
+lift_definition conv_r :: "('a, '\<alpha> \<times> '\<beta>) uexpr \<Rightarrow> ('a, '\<beta> \<times> '\<alpha>) uexpr" ("_\<^sup>-" [999] 999)
+is "\<lambda> e (b1, b2). e (b2, b1)" .
+
+subsection{*Syntax setup*}
+
+nonterminal
+  svid_list and uexpr_list
+
+syntax
+  "_svid_unit"  :: "svid \<Rightarrow> svid_list" ("_")
+  "_svid_list"  :: "svid \<Rightarrow> svid_list \<Rightarrow> svid_list" ("_,/ _")
+  "_uexpr_unit" :: "('a, '\<alpha>) uexpr \<Rightarrow> uexpr_list" ("_" [40] 40)
+  "_uexpr_list" :: "('a, '\<alpha>) uexpr \<Rightarrow> uexpr_list \<Rightarrow> uexpr_list" ("_,/ _" [40,40] 40)
+  "_assignment" :: "svid_list \<Rightarrow> uexprs \<Rightarrow> '\<alpha> hrel"  ("_ :== _ " [60, 60] 52)
+  "_mk_usubst"  :: "svid_list \<Rightarrow> uexprs \<Rightarrow> '\<alpha> usubst"
+
+translations
+  "_mk_usubst \<sigma> (_svid_unit x) v" == "\<sigma>(&x \<mapsto>\<^sub>s v)"
+  "_mk_usubst \<sigma> (_svid_list x xs) (_uexprs v vs)" == "(_mk_usubst (\<sigma>(&x \<mapsto>\<^sub>s v)) xs vs)"
+  "_assignment xs vs" => "CONST assigns_r (_mk_usubst (CONST id) xs vs)"
+  "x :== v" <= "CONST assigns_r (CONST subst_upd (CONST id) (CONST svar x) v)"
+  "x :== v" <= "CONST assigns_r (CONST subst_upd (CONST id) x v)"
+  "x,y :== u,v" <= "CONST assigns_r (CONST subst_upd (CONST subst_upd (CONST id) (CONST svar x) u) (CONST svar y) v)"
+
+adhoc_overloading
+  useq seqr and
+  uskip skip_r
 
 subsection{*While-loop*}
 text{*In order to specify while loops we need a concept that refers to the result of the execution
@@ -56,22 +95,30 @@ text{*In order to specify while loops we need a concept that refers to the resul
       Now we need to reason on the next state space to see if we continue the execution of the body
       or we skip it.*}
 
-definition While :: "'\<alpha> cond \<Rightarrow> '\<alpha> hrel \<Rightarrow> '\<alpha> hrel" ("WHILE (_) DO /(_) OD"  70) where
-"While b C =  (\<nu> X \<bullet> (C ;; X) \<triangleleft> b \<triangleright>\<^sub>r SKIP)"
+definition while :: "'\<alpha> cond \<Rightarrow> '\<alpha> hrel \<Rightarrow> '\<alpha> hrel" ("while\<^sup>\<top> _ do _ od") where
+"while b C =  (\<nu> X \<bullet> (C ;; X) \<triangleleft> b \<triangleright>\<^sub>r II)"
+
+abbreviation while_top :: "'\<alpha> cond \<Rightarrow> '\<alpha> hrel \<Rightarrow> '\<alpha> hrel" ("while _ do _ od") where
+"while b do P od \<equiv> while\<^sup>\<top> b do P od"
+
+definition while_bot :: "'\<alpha> cond \<Rightarrow> '\<alpha> hrel \<Rightarrow> '\<alpha> hrel" ("while\<^sub>\<bottom> _ do _ od") where
+"while\<^sub>\<bottom> b do P od = (\<mu> X \<bullet> (P ;; X) \<triangleleft> b \<triangleright>\<^sub>r II)"
+
+declare while_def [urel_defs]
 
 subsection{*While-loop inv*}
 text {* While loops with invariant decoration *}
 
 definition while_inv :: "'\<alpha> cond \<Rightarrow> '\<alpha> cond \<Rightarrow> '\<alpha> hrel \<Rightarrow> '\<alpha> hrel" ("while _ invr _ do _ od" 70) where
-"while b invr p do S od = WHILE b DO S OD"
+"while b invr p do S od = while\<^sup>\<top> b do S od"
 
 subsection{*assert and assume*}
 
 definition rassume :: "'\<alpha> upred \<Rightarrow> '\<alpha> hrel" ("_\<^sup>\<top>" [999] 999) where
-[urel_defs]: "rassume c = SKIP \<triangleleft> c \<triangleright>\<^sub>r false"
+[urel_defs]: "rassume c = II \<triangleleft> c \<triangleright>\<^sub>r false"
 
 definition rassert :: "'\<alpha> upred \<Rightarrow> '\<alpha> hrel" ("_\<^sub>\<bottom>" [999] 999) where
-[urel_defs]: "rassert c = SKIP \<triangleleft> c \<triangleright>\<^sub>r true"
+[urel_defs]: "rassert c = II \<triangleleft> c \<triangleright>\<^sub>r true"
 
 subsection{*throw*} 
 text{*To model exceptions we need to use the flag OK from UTP.
@@ -111,29 +158,43 @@ is "\<lambda> P b. P (fst b) b" .
 
 lemma call_prog_val: "call \<lbrace>|P|\<rbrace>\<^sub>u = P"
   by (simp add: call_def urel_defs lit.rep_eq Rep_uexpr_inverse)
-nonterminal
-  svid_list and uexpr_list
-
-syntax
-  "_svid_unit"  :: "svid \<Rightarrow> svid_list" ("_")
-  "_svid_list"  :: "svid \<Rightarrow> svid_list \<Rightarrow> svid_list" ("_,/ _")
-  "_uexpr_unit" :: "('a, '\<alpha>) uexpr \<Rightarrow> uexpr_list" ("_" [40] 40)
-  "_uexpr_list" :: "('a, '\<alpha>) uexpr \<Rightarrow> uexpr_list \<Rightarrow> uexpr_list" ("_,/ _" [40,40] 40)
-  "_assignment" :: "svid_list \<Rightarrow> uexprs \<Rightarrow> '\<alpha> hrel"  ("_ :== _ " [60, 60] 52)
-  "_mk_usubst"  :: "svid_list \<Rightarrow> uexprs \<Rightarrow> '\<alpha> usubst"
-
-translations
-  "_mk_usubst \<sigma> (_svid_unit x) v" == "\<sigma>(&x \<mapsto>\<^sub>s v)"
-  "_mk_usubst \<sigma> (_svid_list x xs) (_uexprs v vs)" == "(_mk_usubst (\<sigma>(&x \<mapsto>\<^sub>s v)) xs vs)"
-  "_assignment xs vs" => "CONST assigns_r (_mk_usubst (CONST id) xs vs)"
-  "x :== v" <= "CONST assigns_r (CONST subst_upd (CONST id) (CONST svar x) v)"
-  "x :== v" <= "CONST assigns_r (CONST subst_upd (CONST id) x v)"
-  "x,y :== u,v" <= "CONST assigns_r (CONST subst_upd (CONST subst_upd (CONST id) (CONST svar x) u) (CONST svar y) v)"
 
 notation (latex)
   skip_r  ("\<SKIP>") and
   cond  ("\<IF> _ \<THEN> _ \<ELSE> _"  60) and
-  While  ("\<WHILE> _ \<DO> _ \<OD>"  60)
+  while  ("\<WHILE> _ \<DO> _ \<OD>"  60)
 
+subsection {*Props *}
 
+text {* We describe some properties of relations *}
+
+definition ufunctional :: "('a, 'b) rel \<Rightarrow> bool"
+where "ufunctional R \<longleftrightarrow> II \<sqsubseteq> R\<^sup>- ;; R"
+
+declare ufunctional_def [urel_defs]
+
+definition uinj :: "('a, 'b) rel \<Rightarrow> bool"
+where "uinj R \<longleftrightarrow> II \<sqsubseteq> R ;; R\<^sup>-"
+
+declare uinj_def [urel_defs]
+
+text {* A test is like a precondition, except that it identifies to the postcondition. It
+        forms the basis for Kleene Algebra with Tests (KAT). *}
+
+definition lift_test :: "'\<alpha> cond \<Rightarrow> '\<alpha> hrel" ("\<lceil>_\<rceil>\<^sub>t")
+where "\<lceil>b\<rceil>\<^sub>t = (\<lceil>b\<rceil>\<^sub>< \<and> II)"
+
+declare cond_def [urel_defs]
+declare skip_r_def [urel_defs]
+
+text {* We implement a poor man's version of alphabet restriction that hides a variable within a relation *}
+
+definition rel_var_res :: "'\<alpha> hrel \<Rightarrow> ('a, '\<alpha>) uvar \<Rightarrow> '\<alpha> hrel" (infix "\<restriction>\<^sub>\<alpha>" 80) where
+"P \<restriction>\<^sub>\<alpha> x = (\<exists> $x \<bullet> \<exists> $x\<acute> \<bullet> P)"
+
+declare rel_var_res_def [urel_defs]
+
+-- {* Configuration for UTP tactics (see @{theory utp_tactics}). *}
+
+update_uexpr_rep_eq_thms -- {* Reread @{text rep_eq} theorems. *}
 end
