WP1-Programming-Languages-Semantics/WP11-C-semantics/src/IMP-Lenses/utp/utp_urel_laws.thy
@@ -1,15 +1,15 @@
 section {* UTP variables *}
 
 theory utp_urel_laws
-  imports "../Commands"
+  imports "utp_rel"
 begin
-
+  
 subsection {* Unrestriction Laws *}
 
 lemma unrest_iuvar [unrest]: (*legacy assumes 1:"mwb_lens x"*) 
   "out\<alpha> \<sharp> $x" 
   by (simp add: out\<alpha>_def, transfer, auto)
-
+ 
 lemma unrest_ouvar [unrest]: (*legacy need assumes 1:"mwb_lens x"*) 
   "in\<alpha> \<sharp> $x\<acute>" 
   by (simp add: in\<alpha>_def, transfer, auto)
@@ -18,16 +18,16 @@ lemma unrest_semir_undash [unrest]:
   fixes x :: "('a, '\<alpha>) uvar"
   assumes "$x \<sharp> P"
   shows "$x \<sharp> P ;; Q"
-  using assms by (rel_auto)
+  using assms by transfer (rel_auto) 
 
 lemma unrest_semir_dash [unrest]:
   fixes x :: "('a, '\<alpha>) uvar"
   assumes "$x\<acute> \<sharp> Q"
   shows "$x\<acute> \<sharp> P ;; Q"
-  using assms by (rel_auto)
+  using assms by transfer (rel_auto)
 
 lemma unrest_cond [unrest]:
-  "\<lbrakk> x \<sharp> P; x \<sharp> b; x \<sharp> Q \<rbrakk> \<Longrightarrow> x \<sharp> IF b THEN P ELSE Q"
+  "\<lbrakk> x \<sharp> P; x \<sharp> b; x \<sharp> Q \<rbrakk> \<Longrightarrow> x \<sharp> P \<triangleleft> b \<triangleright> Q "
   unfolding cond_def
   by transfer' (rel_auto)
 
@@ -59,7 +59,7 @@ lemma unrest_post_out_var [unrest]:
   "x \<sharp> p1 \<Longrightarrow> $x\<acute> \<sharp> \<lceil>p1\<rceil>\<^sub>>"
   by (transfer, simp)
 
-(*lemma unrest_convr_out\<alpha> [unrest]:
+lemma unrest_convr_out\<alpha> [unrest]:
   "in\<alpha> \<sharp> p \<Longrightarrow> out\<alpha> \<sharp> p\<^sup>-"
   by (transfer, auto simp add: in\<alpha>_def out\<alpha>_def)
 
@@ -70,20 +70,20 @@ lemma unrest_convr_in\<alpha> [unrest]:
 lemma unrest_in_rel_var_res [unrest]:
   "vwb_lens x \<Longrightarrow> $x \<sharp> (P \<restriction>\<^sub>\<alpha> x)"
   by (simp add: rel_var_res_def unrest)
-
+ 
 lemma unrest_out_rel_var_res [unrest]:
   "vwb_lens x \<Longrightarrow> $x\<acute> \<sharp> (P \<restriction>\<^sub>\<alpha> x)"
-  by (simp add: rel_var_res_def unrest)*)
+  by (simp add: rel_var_res_def unrest)
 
 subsection {* Substitution laws *}
 
 lemma subst_seq_left [usubst]:
   "out\<alpha> \<sharp> \<sigma> \<Longrightarrow> \<sigma> \<dagger> (P ;; Q) = (\<sigma> \<dagger> P) ;; Q"
-  by (rel_auto, (metis (no_types, lifting) Pair_inject surjective_pairing)+)
+  by transfer (rel_auto, (metis (no_types, lifting) Pair_inject surjective_pairing)+)
 
 lemma subst_seq_right [usubst]:
   "in\<alpha> \<sharp> \<sigma> \<Longrightarrow> \<sigma> \<dagger> (P ;; Q) = P ;; (\<sigma> \<dagger> Q)"
-  by (rel_auto, (metis (no_types, lifting) Pair_inject surjective_pairing)+)
+  by transfer (rel_auto, (metis (no_types, lifting) Pair_inject surjective_pairing)+)
 
 text {* The following laws support substitution in heterogeneous relations for polymorphically
   types literal expressions. These cannot be supported more generically due to limitations
@@ -97,7 +97,7 @@ lemma bool_seqr_laws [usubst]:
     "\<And> P Q \<sigma>. \<sigma>($x \<mapsto>\<^sub>s false) \<dagger> (P ;; Q) = \<sigma> \<dagger> (P\<lbrakk>false/$x\<rbrakk> ;; Q)"
     "\<And> P Q \<sigma>. \<sigma>($x\<acute> \<mapsto>\<^sub>s true) \<dagger> (P ;; Q) = \<sigma> \<dagger> (P ;; Q\<lbrakk>true/$x\<acute>\<rbrakk>)"
     "\<And> P Q \<sigma>. \<sigma>($x\<acute> \<mapsto>\<^sub>s false) \<dagger> (P ;; Q) = \<sigma> \<dagger> (P ;; Q\<lbrakk>false/$x\<acute>\<rbrakk>)"
-    by (rel_auto)+
+    by (transfer, rel_auto)+
 
 lemma zero_one_seqr_laws [usubst]:
   fixes x :: "(_ \<Longrightarrow> '\<alpha>)"
@@ -106,23 +106,23 @@ lemma zero_one_seqr_laws [usubst]:
     "\<And> P Q \<sigma>. \<sigma>($x \<mapsto>\<^sub>s 1) \<dagger> (P ;; Q) = \<sigma> \<dagger> (P\<lbrakk>1/$x\<rbrakk> ;; Q)"
     "\<And> P Q \<sigma>. \<sigma>($x\<acute> \<mapsto>\<^sub>s 0) \<dagger> (P ;; Q) = \<sigma> \<dagger> (P ;; Q\<lbrakk>0/$x\<acute>\<rbrakk>)"
     "\<And> P Q \<sigma>. \<sigma>($x\<acute> \<mapsto>\<^sub>s 1) \<dagger> (P ;; Q) = \<sigma> \<dagger> (P ;; Q\<lbrakk>1/$x\<acute>\<rbrakk>)"
-    by (rel_auto)+
+    by (transfer, rel_auto)+
 
 lemma numeral_seqr_laws [usubst]:
   fixes x :: "(_ \<Longrightarrow> '\<alpha>)"
   shows 
     "\<And> P Q \<sigma>. \<sigma>($x \<mapsto>\<^sub>s numeral n) \<dagger> (P ;; Q) = \<sigma> \<dagger> (P\<lbrakk>numeral n/$x\<rbrakk> ;; Q)"
     "\<And> P Q \<sigma>. \<sigma>($x\<acute> \<mapsto>\<^sub>s numeral n) \<dagger> (P ;; Q) = \<sigma> \<dagger> (P ;; Q\<lbrakk>numeral n/$x\<acute>\<rbrakk>)"
-  by (rel_auto)+    
+  by (transfer, rel_auto)+    
 
 lemma usubst_condr [usubst]:
-  "\<sigma> \<dagger> (IF b THEN P ELSE Q) = (IF \<sigma> \<dagger> b THEN \<sigma> \<dagger> P ELSE \<sigma> \<dagger> Q)"
+  "\<sigma> \<dagger> ( P \<triangleleft> b \<triangleright> Q) = (\<sigma> \<dagger> P \<triangleleft> \<sigma> \<dagger> b \<triangleright> \<sigma> \<dagger> Q)"
   unfolding cond_def
-  by transfer' (rel_auto)
+  by rel_auto
  
-(*lemma subst_skip_r [usubst]:
-  "out\<alpha> \<sharp> \<sigma> \<Longrightarrow> \<sigma> \<dagger> SKIP = \<langle>\<lfloor>\<sigma>\<rfloor>\<^sub>s\<rangle>\<^sub>a"
-  by (rel_auto, (metis (mono_tags, lifting) prod.sel(1) sndI surjective_pairing)+)*)
+lemma subst_skip_r [usubst]:
+  "out\<alpha> \<sharp> \<sigma> \<Longrightarrow> \<sigma> \<dagger> II = \<langle>\<lfloor>\<sigma>\<rfloor>\<^sub>s\<rangle>\<^sub>a"
+  by (rel_simp, (metis (mono_tags, lifting) prod.sel(1) sndI surjective_pairing)+)
 
 lemma usubst_upd_in_comp [usubst]:
   "\<sigma>(&in\<alpha>:x \<mapsto>\<^sub>s v) = \<sigma>($x \<mapsto>\<^sub>s v)"
@@ -135,24 +135,24 @@ lemma usubst_upd_out_comp [usubst]:
 lemma subst_lift_upd [usubst]:
   fixes x :: "('a, '\<alpha>) uvar"
   shows "\<lceil>\<sigma>(x \<mapsto>\<^sub>s v)\<rceil>\<^sub>s = \<lceil>\<sigma>\<rceil>\<^sub>s($x \<mapsto>\<^sub>s \<lceil>v\<rceil>\<^sub><)"
-  by (simp add: alpha usubst, simp add: fst_lens_def in\<alpha>_def in_var_def)
+  by (simp add: alpha , simp add: fst_lens_def in\<alpha>_def in_var_def)
 
 lemma subst_drop_upd [usubst]:
   fixes x :: "('a, '\<alpha>) uvar"
   shows "\<lfloor>\<sigma>($x \<mapsto>\<^sub>s v)\<rfloor>\<^sub>s = \<lfloor>\<sigma>\<rfloor>\<^sub>s(x \<mapsto>\<^sub>s \<lfloor>v\<rfloor>\<^sub><)"
-  by (pred_auto, simp add: in\<alpha>_def prod.case_eq_if)
+  by  (pred_simp , simp add: in\<alpha>_def prod.case_eq_if)
 
 lemma subst_lift_pre [usubst]: "\<lceil>\<sigma>\<rceil>\<^sub>s \<dagger> \<lceil>b\<rceil>\<^sub>< = \<lceil>\<sigma> \<dagger> b\<rceil>\<^sub><"
   by (metis apply_subst_ext fst_lens_def fst_vwb_lens in\<alpha>_def)
 
 lemma unrest_usubst_lift_in [unrest]:
   "x \<sharp> P \<Longrightarrow> $x \<sharp> \<lceil>P\<rceil>\<^sub>s"
-  by (pred_auto, auto simp add: unrest_usubst_def in\<alpha>_def)
+  by (pred_simp, auto simp add: unrest_usubst_def in\<alpha>_def)
 
 lemma unrest_usubst_lift_out [unrest]:
   fixes x :: "('a, '\<alpha>) uvar"
   shows "$x\<acute> \<sharp> \<lceil>P\<rceil>\<^sub>s"
-  by (pred_auto, auto simp add: unrest_usubst_def in\<alpha>_def)
+  by (pred_simp, auto simp add: unrest_usubst_def in\<alpha>_def)
 
 subsection {* Relation laws *}
 
@@ -166,43 +166,46 @@ abbreviation falser :: "'\<alpha> hrel" ("false\<^sub>h") where
 "falser \<equiv> false"
 
 lemma drop_pre_inv [simp]: "\<lbrakk> out\<alpha> \<sharp> p \<rbrakk> \<Longrightarrow> \<lceil>\<lfloor>p\<rfloor>\<^sub><\<rceil>\<^sub>< = p"
-  by (pred_auto, auto simp add: out\<alpha>_def lens_create_def fst_lens_def prod.case_eq_if)
-
-
-
-    
+  by (pred_simp, auto simp add: out\<alpha>_def lens_create_def fst_lens_def prod.case_eq_if)
+   
 text {* Quantale laws for relations *}
-    
-(*lemma seq_Sup_distl: "P ;; (\<Sqinter> A) = (\<Sqinter> Q\<in>A. P ;; Q)"
-  by (transfer, auto)
+
+lemma seq_Sup_distl: "P ;; (\<Sqinter> A) = (\<Sqinter> Q\<in>A. P ;; Q)"
+  unfolding SUP_def
+  by (transfer, rel_auto)
     
 lemma seq_Sup_distr: "(\<Sqinter> A) ;; Q = (\<Sqinter> P\<in>A. P ;; Q)"
+  unfolding SUP_def
   by (transfer, auto)
     
 lemma seq_UINF_distl: "P ;; (\<Sqinter> Q\<in>A \<bullet> F(Q)) = (\<Sqinter> Q\<in>A \<bullet> P ;; F(Q))"
-  by (simp add: USUP_as_Sup_collect seq_Sup_distl)
+  apply (simp add: USUP_as_Sup_collect seq_Sup_distl)
+  unfolding SUP_def apply transfer apply auto
+done
 
 lemma seq_UINF_distr: "(\<Sqinter> P\<in>A \<bullet> F(P)) ;; Q = (\<Sqinter> P\<in>A \<bullet> F(P) ;; Q)"
-  by (simp add: USUP_as_Sup_collect seq_Sup_distr)*)
+  apply  (simp add: USUP_as_Sup_collect seq_Sup_distr)
+  unfolding SUP_def apply transfer apply auto
+done
 
 lemma impl_seqr_mono: "\<lbrakk> `P \<Rightarrow> Q`; `R \<Rightarrow> S` \<rbrakk> \<Longrightarrow> `(P ;; R) \<Rightarrow> (Q ;; S)`"
-  by (pred_blast)
+  by transfer (pred_blast)
 
 lemma seqr_mono:
   "\<lbrakk> P\<^sub>1 \<sqsubseteq> P\<^sub>2; Q\<^sub>1 \<sqsubseteq> Q\<^sub>2 \<rbrakk> \<Longrightarrow> (P\<^sub>1 ;; Q\<^sub>1) \<sqsubseteq> (P\<^sub>2 ;; Q\<^sub>2)"
-  by (rel_blast)
+  by transfer (rel_blast)
 
 lemma seqr_monotonic: 
   "\<lbrakk> mono P; mono Q \<rbrakk> \<Longrightarrow> mono (\<lambda> X. P X ;; Q X)"
-  by (simp add: mono_def, rel_blast)
+  by (simp add: mono_def, transfer ,rel_blast)
 
 lemma cond_mono:
-  "\<lbrakk> P\<^sub>1 \<sqsubseteq> P\<^sub>2; Q\<^sub>1 \<sqsubseteq> Q\<^sub>2 \<rbrakk> \<Longrightarrow> (IF b THEN P\<^sub>1 ELSE Q\<^sub>1) \<sqsubseteq> (IF b THEN P\<^sub>2 ELSE Q\<^sub>2)"
+  "\<lbrakk> P\<^sub>1 \<sqsubseteq> P\<^sub>2; Q\<^sub>1 \<sqsubseteq> Q\<^sub>2 \<rbrakk> \<Longrightarrow> (P\<^sub>1 \<triangleleft> b \<triangleright> Q\<^sub>1) \<sqsubseteq> (P\<^sub>2 \<triangleleft> b \<triangleright> Q\<^sub>2)"
   unfolding cond_def
-  by (rel_auto)
+  by transfer (rel_auto)
 
 lemma cond_monotonic:
-  "\<lbrakk> mono P; mono Q \<rbrakk> \<Longrightarrow> mono (\<lambda> X. IF b THEN P X ELSE Q X)"
+  "\<lbrakk> mono P; mono Q \<rbrakk> \<Longrightarrow> mono (\<lambda> X. P X \<triangleleft> b \<triangleright> Q X)"
   unfolding cond_def
   by (simp add: mono_def, rel_blast)
 
@@ -210,48 +213,46 @@ lemma spec_refine:
   "Q \<sqsubseteq> (P \<and> R) \<Longrightarrow> (P \<Rightarrow> Q) \<sqsubseteq> R"
   by (rel_auto)
 
-(*lemma cond_skip: "out\<alpha> \<sharp> b \<Longrightarrow> (b \<and> II) = (II \<and> b\<^sup>-)"
-  by (rel_auto)*)
+lemma cond_skip: "out\<alpha> \<sharp> b \<Longrightarrow> (b \<and> II) = (II \<and> b\<^sup>-)"
+  by (rel_auto)
 
 
 lemma assigns_subst [usubst]:
   "\<lceil>\<sigma>\<rceil>\<^sub>s \<dagger> \<langle>\<rho>\<rangle>\<^sub>a = \<langle>\<rho> \<circ> \<sigma>\<rangle>\<^sub>a"
-  by (rel_auto)
+  by transfer (rel_auto)
 
 lemma assigns_r_comp: "(\<langle>\<sigma>\<rangle>\<^sub>a ;; P) = (\<lceil>\<sigma>\<rceil>\<^sub>s \<dagger> P)"
-  by rel_auto
+  by transfer rel_auto
 
 lemma assigns_r_feasible:
   "(\<langle>\<sigma>\<rangle>\<^sub>a ;; true) = true"
-  by (rel_auto)
+  by (simp add: assigns_r_comp subst_true)
 
-(*lemma assign_subst [usubst]:
-  "\<lbrakk> mwb_lens x; mwb_lens y \<rbrakk> \<Longrightarrow> [$x \<mapsto>\<^sub>s \<lceil>u\<rceil>\<^sub><] \<dagger> (y := v) = (x, y := u, [x \<mapsto>\<^sub>s u] \<dagger> v)"
+lemma assign_subst [usubst]:
+  "\<lbrakk> mwb_lens x; mwb_lens y \<rbrakk> \<Longrightarrow> [$x \<mapsto>\<^sub>s \<lceil>u\<rceil>\<^sub><] \<dagger> (y :== v) = (x, y :== u, [x \<mapsto>\<^sub>s u] \<dagger> v)"
   by rel_auto
 
-lemma assigns_idem: "mwb_lens x \<Longrightarrow> (x,x := u,v) = (x := v)"
-  by (simp add: usubst)*)
+lemma assigns_idem: "mwb_lens x \<Longrightarrow> (x,x :== u,v) = (x :== v)"
+  by (simp add: usubst)
 
 lemma assigns_comp: "(\<langle>f\<rangle>\<^sub>a ;; \<langle>g\<rangle>\<^sub>a) = \<langle>g \<circ> f\<rangle>\<^sub>a"
   by (simp add: assigns_r_comp usubst)
 
-(*lemma assigns_r_conv:
+lemma assigns_r_conv:
   "bij f \<Longrightarrow> \<langle>f\<rangle>\<^sub>a\<^sup>- = \<langle>inv f\<rangle>\<^sub>a"
-  by (rel_auto, simp_all add: bij_is_inj bij_is_surj surj_f_inv_f)
+  by transfer (rel_auto, simp_all add: bij_is_inj bij_is_surj surj_f_inv_f)
 
 lemma assign_pred_transfer:
   fixes x :: "('a, '\<alpha>) uvar"
   assumes "$x \<sharp> b" "out\<alpha> \<sharp> b"
-  shows "(b \<and> x := v) = (x := v \<and> b\<^sup>-)"
-  using assms by (rel_blast)*)
+  shows "(b \<and> x :== v) = (x :== v \<and> b\<^sup>-)"
+  using assms by rel_blast
 
-
-
-(*lemma assigns_r_ufunc: "ufunctional \<langle>f\<rangle>\<^sub>a"
+lemma assigns_r_ufunc: "ufunctional \<langle>f\<rangle>\<^sub>a"
   by (rel_auto)
 
 lemma assigns_r_uinj: "inj f \<Longrightarrow> uinj \<langle>f\<rangle>\<^sub>a"
-  by (rel_auto, simp add: inj_eq)
+  by (rel_simp, simp add: inj_eq)
 
 lemma assigns_r_swap_uinj:
   "\<lbrakk> vwb_lens x; vwb_lens y; x \<bowtie> y \<rbrakk> \<Longrightarrow> uinj (x,y :== &y,&x)"
@@ -260,8 +261,6 @@ lemma assigns_r_swap_uinj:
 lemma skip_r_unfold:
   "vwb_lens x \<Longrightarrow> II = ($x\<acute> =\<^sub>u $x \<and> II\<restriction>\<^sub>\<alpha>x)"
   by (rel_auto, metis mwb_lens.put_put vwb_lens_mwb vwb_lens_wb wb_lens.get_put)
-
-
 
 lemma skip_ra_unfold:
   "II\<^bsub>x;y\<^esub> = ($x\<acute> =\<^sub>u $x \<and> II\<^bsub>y\<^esub>)"
@@ -275,7 +274,7 @@ lemma skip_res_as_ra:
 done
 
 lemma assign_unfold:
-  "vwb_lens x \<Longrightarrow> (x := v) = ($x\<acute> =\<^sub>u \<lceil>v\<rceil>\<^sub>< \<and> II\<restriction>\<^sub>\<alpha>x)"
+  "vwb_lens x \<Longrightarrow> (x :== v) = ($x\<acute> =\<^sub>u \<lceil>v\<rceil>\<^sub>< \<and> II\<restriction>\<^sub>\<alpha>x)"
   apply (rel_auto, auto simp add: comp_def)
   using vwb_lens.put_eq by fastforce
 
@@ -286,8 +285,6 @@ lemma seqr_and_distr_ufunc:
 lemma seqr_and_distl_uinj:
   "uinj R \<Longrightarrow> ((P \<and> Q) ;; R) = ((P ;; R) \<and> (Q ;; R))"
   by (rel_auto)
-*)
-
 
 theorem precond_equiv:
   "P = (P ;; true) \<longleftrightarrow> (out\<alpha> \<sharp> P)"
@@ -316,7 +313,7 @@ done
 
 subsection {* Converse laws *}
 
-(*lemma convr_invol [simp]: "p\<^sup>-\<^sup>- = p"
+lemma convr_invol [simp]: "p\<^sup>-\<^sup>- = p"
   by pred_auto
 
 lemma lit_convr [simp]: "\<guillemotleft>v\<guillemotright>\<^sup>- = \<guillemotleft>v\<guillemotright>"
@@ -360,7 +357,7 @@ lemma post_convr [simp]: "\<lceil>p\<rceil>\<^sub>>\<^sup>- = \<lceil>p\<rceil>\
   by (rel_auto)
 
 theorem seqr_pre_transfer: "in\<alpha> \<sharp> q \<Longrightarrow> ((P \<and> q) ;; R) = (P ;; (q\<^sup>- \<and> R))"
-  by (rel_auto)*)
+  by (rel_auto)
 
 theorem seqr_pre_transfer':
   "((P \<and> \<lceil>q\<rceil>\<^sub>>) ;; R) = (P ;; (\<lceil>q\<rceil>\<^sub>< \<and> R))"
@@ -374,8 +371,8 @@ lemma seqr_post_var_out:
   shows "(P ;; (Q \<and> $x\<acute>)) = ((P ;; Q) \<and> $x\<acute>)"
   by (rel_auto)
 
-(*theorem seqr_post_transfer: "out\<alpha> \<sharp> q \<Longrightarrow> (P ;; (q \<and> R)) = ((P \<and> q\<^sup>-) ;; R)"
-  by (simp add: seqr_pre_transfer unrest_convr_in\<alpha>)*) 
+theorem seqr_post_transfer: "out\<alpha> \<sharp> q \<Longrightarrow> (P ;; (q \<and> R)) = ((P \<and> q\<^sup>-) ;; R)"
+  by (simp add: seqr_pre_transfer unrest_convr_in\<alpha>) 
 
 lemma seqr_pre_out: "out\<alpha> \<sharp> p \<Longrightarrow> ((p \<and> Q) ;; R) = (p \<and> (Q ;; R))"
   by (rel_blast)
@@ -399,6 +396,136 @@ lemma shEx_lift_seq_1 [uquant_lift]:
 lemma shEx_lift_seq_2 [uquant_lift]:
   "(P ;; (\<^bold>\<exists> x \<bullet> Q x)) = (\<^bold>\<exists> x \<bullet> (P ;; Q x))"
   by pred_auto
+
+subsection {* Relational unrestriction *}
+
+text {* Relational unrestriction states that a variable is unchanged by a relation. Eventually
+  I'd also like to have it state that the relation also does not depend on the variable's
+  initial value, but I'm not sure how to state that yet. For now we represent this by
+  the parametric healthiness condition RID. *}
+
+definition RID :: "('a, '\<alpha>) uvar \<Rightarrow> '\<alpha> hrel \<Rightarrow> '\<alpha> hrel"
+where "RID x P = ((\<exists> $x \<bullet> \<exists> $x\<acute> \<bullet> P) \<and> $x\<acute> =\<^sub>u $x)"
+
+declare RID_def [urel_defs]
+
+lemma RID_idem:
+  "mwb_lens x \<Longrightarrow> RID(x)(RID(x)(P)) = RID(x)(P)"
+  by (rel_auto)
+
+lemma RID_mono:
+  "P \<sqsubseteq> Q \<Longrightarrow> RID(x)(P) \<sqsubseteq> RID(x)(Q)"
+  by (rel_auto)
+
+lemma RID_skip_r:
+  "vwb_lens x \<Longrightarrow> RID(x)(II) = II"
+  apply (rel_auto) using vwb_lens.put_eq by fastforce
+
+lemma RID_disj:
+  "RID(x)(P \<or> Q) = (RID(x)(P) \<or> RID(x)(Q))"
+  by (rel_auto)
+
+lemma RID_conj:
+  "vwb_lens x \<Longrightarrow> RID(x)(RID(x)(P) \<and> RID(x)(Q)) = (RID(x)(P) \<and> RID(x)(Q))"
+  by (rel_auto)
+
+lemma RID_assigns_r_diff:
+  "\<lbrakk> vwb_lens x; x \<sharp> \<sigma> \<rbrakk> \<Longrightarrow> RID(x)(\<langle>\<sigma>\<rangle>\<^sub>a) = \<langle>\<sigma>\<rangle>\<^sub>a"
+  apply (rel_auto)
+  apply (metis vwb_lens.put_eq)
+  apply (metis vwb_lens_wb wb_lens.get_put wb_lens_weak weak_lens.put_get)
+done
+
+lemma RID_assign_r_same:
+  "vwb_lens x \<Longrightarrow> RID(x)(x :== v) = II"
+  apply (rel_auto)
+  using vwb_lens.put_eq apply fastforce
+done
+
+lemma RID_seq_left:
+  assumes "vwb_lens x"
+  shows "RID(x)(RID(x)(P) ;; Q) = (RID(x)(P) ;; RID(x)(Q))"
+proof -
+  have "RID(x)(RID(x)(P) ;; Q) = ((\<exists> $x \<bullet> \<exists> $x\<acute> \<bullet> ((\<exists> $x \<bullet> \<exists> $x\<acute> \<bullet> P) \<and> $x\<acute> =\<^sub>u $x) ;; Q) \<and> $x\<acute> =\<^sub>u $x)"
+    by (simp add: RID_def usubst)
+  also from assms have "... = ((((\<exists> $x \<bullet> \<exists> $x\<acute> \<bullet> P) \<and> (\<exists> $x \<bullet> $x\<acute> =\<^sub>u $x)) ;; (\<exists> $x\<acute> \<bullet> Q)) \<and> $x\<acute> =\<^sub>u $x)"
+    by (rel_auto)
+  also from assms have "... = (((\<exists> $x \<bullet> \<exists> $x\<acute> \<bullet> P) ;; (\<exists> $x \<bullet> \<exists> $x\<acute> \<bullet> Q)) \<and> $x\<acute> =\<^sub>u $x)"
+    apply (rel_auto)
+    apply (metis vwb_lens.put_eq)
+    apply (metis mwb_lens.put_put vwb_lens_mwb)
+  done
+  also from assms have "... = ((((\<exists> $x \<bullet> \<exists> $x\<acute> \<bullet> P) \<and> $x\<acute> =\<^sub>u $x) ;; (\<exists> $x \<bullet> \<exists> $x\<acute> \<bullet> Q)) \<and> $x\<acute> =\<^sub>u $x)"
+    by (rel_simp, metis (full_types) mwb_lens.put_put vwb_lens_def wb_lens_weak weak_lens.put_get)
+  also have "... = ((((\<exists> $x \<bullet> \<exists> $x\<acute> \<bullet> P) \<and> $x\<acute> =\<^sub>u $x) ;; ((\<exists> $x \<bullet> \<exists> $x\<acute> \<bullet> Q) \<and> $x\<acute> =\<^sub>u $x)) \<and> $x\<acute> =\<^sub>u $x)"
+    by (rel_simp, fastforce)
+  also have "... = ((((\<exists> $x \<bullet> \<exists> $x\<acute> \<bullet> P) \<and> $x\<acute> =\<^sub>u $x) ;; ((\<exists> $x \<bullet> \<exists> $x\<acute> \<bullet> Q) \<and> $x\<acute> =\<^sub>u $x)))"
+    by (rel_auto)
+  also have "... = (RID(x)(P) ;; RID(x)(Q))"
+    by (rel_auto)
+  finally show ?thesis .
+qed
+
+lemma RID_seq_right:
+  assumes "vwb_lens x"
+  shows "RID(x)(P ;; RID(x)(Q)) = (RID(x)(P) ;; RID(x)(Q))"
+proof -
+  have "RID(x)(P ;; RID(x)(Q)) = ((\<exists> $x \<bullet> \<exists> $x\<acute> \<bullet> P ;; ((\<exists> $x \<bullet> \<exists> $x\<acute> \<bullet> Q) \<and> $x\<acute> =\<^sub>u $x)) \<and> $x\<acute> =\<^sub>u $x)"
+    by (simp add: RID_def usubst)
+  also from assms have "... = (((\<exists> $x \<bullet>  P) ;; (\<exists> $x \<bullet> \<exists> $x\<acute> \<bullet> Q) \<and> (\<exists> $x\<acute> \<bullet> $x\<acute> =\<^sub>u $x)) \<and> $x\<acute> =\<^sub>u $x)"
+    by (rel_auto)
+  also from assms have "... = (((\<exists> $x \<bullet> \<exists> $x\<acute> \<bullet> P) ;; (\<exists> $x \<bullet> \<exists> $x\<acute> \<bullet> Q)) \<and> $x\<acute> =\<^sub>u $x)"
+    apply (rel_auto)
+    apply (metis vwb_lens.put_eq)
+    apply (metis mwb_lens.put_put vwb_lens_mwb)
+  done
+  also from assms have "... = ((((\<exists> $x \<bullet> \<exists> $x\<acute> \<bullet> P) \<and> $x\<acute> =\<^sub>u $x) ;; (\<exists> $x \<bullet> \<exists> $x\<acute> \<bullet> Q)) \<and> $x\<acute> =\<^sub>u $x)"
+    by (rel_simp, metis (full_types) mwb_lens.put_put vwb_lens_def wb_lens_weak weak_lens.put_get)
+  also have "... = ((((\<exists> $x \<bullet> \<exists> $x\<acute> \<bullet> P) \<and> $x\<acute> =\<^sub>u $x) ;; ((\<exists> $x \<bullet> \<exists> $x\<acute> \<bullet> Q) \<and> $x\<acute> =\<^sub>u $x)) \<and> $x\<acute> =\<^sub>u $x)"
+    by (rel_simp, fastforce)
+  also have "... = ((((\<exists> $x \<bullet> \<exists> $x\<acute> \<bullet> P) \<and> $x\<acute> =\<^sub>u $x) ;; ((\<exists> $x \<bullet> \<exists> $x\<acute> \<bullet> Q) \<and> $x\<acute> =\<^sub>u $x)))"
+    by (rel_auto)
+  also have "... = (RID(x)(P) ;; RID(x)(Q))"
+    by (rel_auto)
+  finally show ?thesis .
+qed
+
+definition unrest_relation :: "('a, '\<alpha>) uvar \<Rightarrow> '\<alpha> hrel \<Rightarrow> bool" (infix "\<sharp>\<sharp>" 20)
+where "(x \<sharp>\<sharp> P) \<longleftrightarrow> (P = RID(x)(P))"
+
+declare unrest_relation_def [urel_defs]
+
+lemma skip_r_runrest [unrest]:
+  "vwb_lens x \<Longrightarrow> x \<sharp>\<sharp> II"
+  by (simp add: RID_skip_r unrest_relation_def)
+
+lemma assigns_r_runrest:
+  "\<lbrakk> vwb_lens x; x \<sharp> \<sigma> \<rbrakk> \<Longrightarrow> x \<sharp>\<sharp> \<langle>\<sigma>\<rangle>\<^sub>a"
+  by (simp add: RID_assigns_r_diff unrest_relation_def)
+
+lemma seq_r_runrest [unrest]:
+  assumes "vwb_lens x" "x \<sharp>\<sharp> P" "x \<sharp>\<sharp> Q"
+  shows "x \<sharp>\<sharp> (P ;; Q)"
+  by (metis RID_seq_left assms unrest_relation_def)
+
+lemma false_runrest [unrest]: "x \<sharp>\<sharp> false"
+  by (rel_auto)
+
+lemma and_runrest [unrest]: "\<lbrakk> vwb_lens x; x \<sharp>\<sharp> P; x \<sharp>\<sharp> Q \<rbrakk> \<Longrightarrow> x \<sharp>\<sharp> (P \<and> Q)"
+  by (metis RID_conj unrest_relation_def)
+
+lemma or_runrest [unrest]: "\<lbrakk> x \<sharp>\<sharp> P; x \<sharp>\<sharp> Q \<rbrakk> \<Longrightarrow> x \<sharp>\<sharp> (P \<or> Q)"
+  by (simp add: RID_disj unrest_relation_def)
+
+subsection {* Alphabet laws *}
+
+lemma aext_cond [alpha]:
+  "(P \<triangleleft> b \<triangleright> Q) \<oplus>\<^sub>p a = ((P \<oplus>\<^sub>p a) \<triangleleft>(b \<oplus>\<^sub>p a)\<triangleright>(Q \<oplus>\<^sub>p a))"
+  by (rel_auto)
+
+lemma aext_seq [alpha]:
+  "wb_lens a \<Longrightarrow> ((P ;; Q) \<oplus>\<^sub>p (a \<times>\<^sub>L a)) = ((P \<oplus>\<^sub>p (a \<times>\<^sub>L a)) ;; (Q \<oplus>\<^sub>p (a \<times>\<^sub>L a)))"
+  by (rel_simp, metis wb_lens_weak weak_lens.put_get)
 
 
 end
