WP1-Programming-Languages-Semantics/WP11-C-semantics/src/IMP-Lenses/Algebraic_Laws.thy
@@ -7,7 +7,7 @@ text{*In this section we introduce the semantic rules related to the different
       language, and this before any deductive proof verification activity or formal testing.*}
 
 theory Algebraic_Laws
-imports Commands "utp/utp_urel_laws"
+imports "utp/utp_urel_laws"
 begin
 
 named_theorems symbolic_exec and symbolic_exec_assign_uop and symbolic_exec_assign_bop and 
@@ -20,28 +20,28 @@ text{*In this section we introduce the algebraic laws of programming related to 
       statement.*}
 
 lemma seqr_left_unit [simp, symbolic_exec_ex]:
-  "SKIP ;; P = P"
+  "II ;; P = P"
   by rel_auto
 
 lemma seqr_right_unit [simp, symbolic_exec_ex]:
-  "P ;; SKIP = P"
+  "P ;; II = P"
   by rel_auto
 
-lemma pre_skip_post: "(\<lceil>b\<rceil>\<^sub>< \<and> SKIP) = (SKIP \<and> \<lceil>b\<rceil>\<^sub>>)"
+lemma pre_skip_post: "(\<lceil>b\<rceil>\<^sub>< \<and> II) = (II \<and> \<lceil>b\<rceil>\<^sub>>)"
   by rel_auto
 
 lemma skip_var:
   fixes x :: "(bool, '\<alpha>) uvar"
-  shows "($x \<and> SKIP) = (SKIP \<and> $x\<acute>)"
+  shows "($x \<and> II) = (II \<and> $x\<acute>)"
   by rel_auto
 
 lemma assign_r_alt_def [symbolic_exec]:
   fixes x :: "('a, '\<alpha>) uvar"
-  shows "x :== v = SKIP\<lbrakk>\<lceil>v\<rceil>\<^sub></$x\<rbrakk>"
+  shows "x :== v = II\<lbrakk>\<lceil>v\<rceil>\<^sub></$x\<rbrakk>"
   by rel_auto
 
 lemma skip_r_alpha_eq:
-  "SKIP = ($\<Sigma>\<acute> =\<^sub>u $\<Sigma>)"
+  "II = ($\<Sigma>\<acute> =\<^sub>u $\<Sigma>)"
   by rel_auto
 
 subsection {*Assignment Laws*}
@@ -68,12 +68,6 @@ lemma assign_test[symbolic_exec]:
   using 1   
   by (simp add: assigns_comp subst_upd_comp subst_lit usubst_upd_idem)
 
-
-lemma "mwb_lens x \<Longrightarrow> `x :== \<guillemotleft>1::int\<guillemotright> ;; x :== \<guillemotleft>3::int\<guillemotright>` = (`&x =\<^sub>u \<guillemotleft>3\<guillemotright>`)" 
-  apply rel_auto
-apply (meson mwb_lens_weak weak_lens.view_determination)
-by (metis mwb_lens_weak odd_nonzero weak_lens.put_get)
-
 lemma assign_r_comp[symbolic_exec]: 
   "(x :== u ;; P) = P\<lbrakk>\<lceil>u\<rceil>\<^sub></$x\<rbrakk>" 
   by (simp add: assigns_r_comp usubst)
@@ -93,8 +87,8 @@ lemma assign_commute:
 lemma assign_cond:
   fixes x :: "('a, '\<alpha>) uvar"
   assumes "out\<alpha> \<sharp> b"
-  shows "(x :== e ;; (IF b THEN P ELSE Q)) = 
-         (IF (b\<lbrakk>\<lceil>e\<rceil>\<^sub></$x\<rbrakk>) THEN (x :== e ;; P) ELSE (x :== e ;; Q))"
+  shows "(x :== e ;; (P \<triangleleft> b \<triangleright> Q)) = 
+         ((x :== e ;; P) \<triangleleft>(b\<lbrakk>\<lceil>e\<rceil>\<^sub></$x\<rbrakk>)\<triangleright> (x :== e ;; Q))"
   by rel_auto
 
 lemma assign_rcond[symbolic_exec]:
@@ -170,15 +164,15 @@ lemma assign_qtop4[symbolic_exec_assign_qtop]:
   by rel_auto
 
 lemma assign_cond_seqr_dist[symbolic_exec]:
-  "(IF (b\<lbrakk>\<lceil>e\<rceil>\<^sub></$v\<rbrakk>) THEN (v:== e ;; P) ELSE (v:== e ;; Q)) = 
-   (v:== e ;; IF b THEN P ELSE Q)" 
+  "((v:== e ;; P) \<triangleleft> (b\<lbrakk>\<lceil>e\<rceil>\<^sub></$v\<rbrakk>) \<triangleright> (v:== e ;; Q)) = 
+   (v:== e ;; P \<triangleleft> b \<triangleright> Q)" 
   by rel_auto
 
 text {*In the sequel we find assignment laws proposed by Hoare*}
 
 lemma assign_vwb_skip:
   assumes 1: "vwb_lens v"
-  shows "(v:== &v) = SKIP"
+  shows "(v:== &v) = II"
   by (simp add: assms skip_r_def usubst_upd_var_id)
 
 lemma assign_simultaneous:
@@ -273,7 +267,15 @@ lemma assign_cond_If_uop[symbolic_exec_assign_uop]:
          (v:== uop F (&v)) \<triangleleft>uop F (&v)\<triangleright>\<^sub>r (v:== uop G (&v))) =
          (v:== trop If (uop F E) (uop F E) (uop G E))" 
   using 1
-  by rel_auto
+proof (rel_simp, transfer)
+  fix a :: 'a and b :: 'a and va :: "bool \<Longrightarrow> 'a" and Fa :: "bool \<Rightarrow> bool" and Ea :: "'a \<Rightarrow> bool" and Ga :: "bool \<Rightarrow> bool"
+  have "Fa (Ea a) \<longrightarrow> (Fa (Ea a) \<and> b = put\<^bsub>va\<^esub> a (Fa (Ea a)) \<or> \<not> Fa (Ea a) \<and> b = put\<^bsub>va\<^esub> a (Ga (Ea a))) \<and> b = put\<^bsub>va\<^esub> a (Fa (Ea a) \<or> \<not> Fa (Ea a) \<and> Ga (Ea a)) \<or> \<not> b = put\<^bsub>va\<^esub> a (Fa (Ea a) \<or> \<not> Fa (Ea a) \<and> Ga (Ea a)) \<and> (\<not> Fa (Ea a) \<or> \<not> b = put\<^bsub>va\<^esub> a (Fa (Ea a)))"
+    by presburger
+  then have "\<not> ((\<not> Fa (Ea a) \<or> \<not> b = put\<^bsub>va\<^esub> a (Fa (Ea a))) \<and> (Fa (Ea a) \<or> \<not> b = put\<^bsub>va\<^esub> a (Ga (Ea a)))) = (b = put\<^bsub>va\<^esub> a (Fa (Ea a) \<or> \<not> Fa (Ea a) \<and> Ga (Ea a)))"
+    by fastforce
+  then show "(Fa (Ea a) \<and> b = put\<^bsub>va\<^esub> a (Fa (Ea a)) \<or> \<not> Fa (Ea a) \<and> b = put\<^bsub>va\<^esub> a (Ga (Ea a))) = (b = put\<^bsub>va\<^esub> a (Fa (Ea a) \<or> \<not> Fa (Ea a) \<and> Ga (Ea a)))"
+    by meson
+qed 
 
 lemma assign_cond_If_bop[symbolic_exec_assign_bop]:
   assumes 1: "mwb_lens v" and 2:"v \<sharp> exp"
@@ -281,7 +283,15 @@ lemma assign_cond_If_bop[symbolic_exec_assign_bop]:
           (v:== (bop F exp (&v))) \<triangleleft>bop F exp (&v)\<triangleright>\<^sub>r (v:== (bop G exp (&v)))) =
          (v:== (trop If (bop F exp E) (bop F exp E) (bop G exp E)))" 
   using 1 2
-  by rel_auto
+proof (rel_simp, transfer)
+  fix a :: 'a and b :: 'a and va :: "bool \<Longrightarrow> 'a" and Fa :: "bool \<Rightarrow> bool" and Ea :: "'a \<Rightarrow> bool" and Ga :: "bool \<Rightarrow> bool"
+  have "Fa (Ea a) \<longrightarrow> (Fa (Ea a) \<and> b = put\<^bsub>va\<^esub> a (Fa (Ea a)) \<or> \<not> Fa (Ea a) \<and> b = put\<^bsub>va\<^esub> a (Ga (Ea a))) \<and> b = put\<^bsub>va\<^esub> a (Fa (Ea a) \<or> \<not> Fa (Ea a) \<and> Ga (Ea a)) \<or> \<not> b = put\<^bsub>va\<^esub> a (Fa (Ea a) \<or> \<not> Fa (Ea a) \<and> Ga (Ea a)) \<and> (\<not> Fa (Ea a) \<or> \<not> b = put\<^bsub>va\<^esub> a (Fa (Ea a)))"
+    by presburger
+  then have "\<not> ((\<not> Fa (Ea a) \<or> \<not> b = put\<^bsub>va\<^esub> a (Fa (Ea a))) \<and> (Fa (Ea a) \<or> \<not> b = put\<^bsub>va\<^esub> a (Ga (Ea a)))) = (b = put\<^bsub>va\<^esub> a (Fa (Ea a) \<or> \<not> Fa (Ea a) \<and> Ga (Ea a)))"
+    by fastforce
+  then show "(Fa (Ea a) \<and> b = put\<^bsub>va\<^esub> a (Fa (Ea a)) \<or> \<not> Fa (Ea a) \<and> b = put\<^bsub>va\<^esub> a (Ga (Ea a))) = (b = put\<^bsub>va\<^esub> a (Fa (Ea a) \<or> \<not> Fa (Ea a) \<and> Ga (Ea a)))"
+    by meson
+qed 
 
 lemma assign_cond_If_bop1[symbolic_exec_assign_bop]:
   assumes 1: "mwb_lens v" and 2:"v \<sharp> exp"
@@ -289,7 +299,15 @@ lemma assign_cond_If_bop1[symbolic_exec_assign_bop]:
           (v:== (bop F (&v) exp)) \<triangleleft>bop F (&v) exp\<triangleright>\<^sub>r (v:== (bop G (&v) exp))) =
          (v:== (trop If (bop F E exp) (bop F E exp) (bop G E exp)))" 
   using 1 2
-  by rel_auto
+proof (rel_simp, transfer)
+  fix a :: 'a and b :: 'a and va :: "bool \<Longrightarrow> 'a" and Fa :: "bool \<Rightarrow> bool" and Ea :: "'a \<Rightarrow> bool" and Ga :: "bool \<Rightarrow> bool"
+  have "Fa (Ea a) \<longrightarrow> (Fa (Ea a) \<and> b = put\<^bsub>va\<^esub> a (Fa (Ea a)) \<or> \<not> Fa (Ea a) \<and> b = put\<^bsub>va\<^esub> a (Ga (Ea a))) \<and> b = put\<^bsub>va\<^esub> a (Fa (Ea a) \<or> \<not> Fa (Ea a) \<and> Ga (Ea a)) \<or> \<not> b = put\<^bsub>va\<^esub> a (Fa (Ea a) \<or> \<not> Fa (Ea a) \<and> Ga (Ea a)) \<and> (\<not> Fa (Ea a) \<or> \<not> b = put\<^bsub>va\<^esub> a (Fa (Ea a)))"
+    by presburger
+  then have "\<not> ((\<not> Fa (Ea a) \<or> \<not> b = put\<^bsub>va\<^esub> a (Fa (Ea a))) \<and> (Fa (Ea a) \<or> \<not> b = put\<^bsub>va\<^esub> a (Ga (Ea a)))) = (b = put\<^bsub>va\<^esub> a (Fa (Ea a) \<or> \<not> Fa (Ea a) \<and> Ga (Ea a)))"
+    by fastforce
+  then show "(Fa (Ea a) \<and> b = put\<^bsub>va\<^esub> a (Fa (Ea a)) \<or> \<not> Fa (Ea a) \<and> b = put\<^bsub>va\<^esub> a (Ga (Ea a))) = (b = put\<^bsub>va\<^esub> a (Fa (Ea a) \<or> \<not> Fa (Ea a) \<and> Ga (Ea a)))"
+    by meson
+qed 
 
 lemma assign_cond_If_bop2[symbolic_exec_assign_bop]:
   assumes 1: "mwb_lens v" and 2:"v \<sharp> exp1" and 3:"v \<sharp> exp2"
@@ -297,7 +315,15 @@ lemma assign_cond_If_bop2[symbolic_exec_assign_bop]:
           (v:== (bop F (&v) exp1)) \<triangleleft>bop F (&v) exp1\<triangleright>\<^sub>r (v:== (bop G (&v) exp2))) =
          (v:== (trop If (bop F E exp1) (bop F E exp1) (bop G E exp2)))" 
   using 1 2 3
-  by rel_auto
+proof (rel_simp, transfer)
+  fix a :: 'a and b :: 'a and va :: "bool \<Longrightarrow> 'a" and Fa :: "bool \<Rightarrow> bool" and Ea :: "'a \<Rightarrow> bool" and Ga :: "bool \<Rightarrow> bool"
+  have "Fa (Ea a) \<longrightarrow> (Fa (Ea a) \<and> b = put\<^bsub>va\<^esub> a (Fa (Ea a)) \<or> \<not> Fa (Ea a) \<and> b = put\<^bsub>va\<^esub> a (Ga (Ea a))) \<and> b = put\<^bsub>va\<^esub> a (Fa (Ea a) \<or> \<not> Fa (Ea a) \<and> Ga (Ea a)) \<or> \<not> b = put\<^bsub>va\<^esub> a (Fa (Ea a) \<or> \<not> Fa (Ea a) \<and> Ga (Ea a)) \<and> (\<not> Fa (Ea a) \<or> \<not> b = put\<^bsub>va\<^esub> a (Fa (Ea a)))"
+    by presburger
+  then have "\<not> ((\<not> Fa (Ea a) \<or> \<not> b = put\<^bsub>va\<^esub> a (Fa (Ea a))) \<and> (Fa (Ea a) \<or> \<not> b = put\<^bsub>va\<^esub> a (Ga (Ea a)))) = (b = put\<^bsub>va\<^esub> a (Fa (Ea a) \<or> \<not> Fa (Ea a) \<and> Ga (Ea a)))"
+    by fastforce
+  then show "(Fa (Ea a) \<and> b = put\<^bsub>va\<^esub> a (Fa (Ea a)) \<or> \<not> Fa (Ea a) \<and> b = put\<^bsub>va\<^esub> a (Ga (Ea a))) = (b = put\<^bsub>va\<^esub> a (Fa (Ea a) \<or> \<not> Fa (Ea a) \<and> Ga (Ea a)))"
+    by meson
+qed 
 
 lemma assign_cond_If_bop4[symbolic_exec_assign_bop]:
   assumes 1: "mwb_lens v" and 2:"v \<sharp> exp1" and 3:"v \<sharp> exp2"
@@ -305,7 +331,15 @@ lemma assign_cond_If_bop4[symbolic_exec_assign_bop]:
           (v:== (bop F (&v) exp1)) \<triangleleft>bop F (&v) exp1\<triangleright>\<^sub>r (v:== (bop G exp2 (&v)))) =
          (v:== (trop If (bop F E exp1) (bop F E exp1) (bop G exp2 E)))" 
   using 1 2 3
-  by rel_auto
+proof (rel_simp, transfer)
+  fix a :: 'a and b :: 'a and va :: "bool \<Longrightarrow> 'a" and Fa :: "bool \<Rightarrow> bool" and Ea :: "'a \<Rightarrow> bool" and Ga :: "bool \<Rightarrow> bool"
+  have "Fa (Ea a) \<longrightarrow> (Fa (Ea a) \<and> b = put\<^bsub>va\<^esub> a (Fa (Ea a)) \<or> \<not> Fa (Ea a) \<and> b = put\<^bsub>va\<^esub> a (Ga (Ea a))) \<and> b = put\<^bsub>va\<^esub> a (Fa (Ea a) \<or> \<not> Fa (Ea a) \<and> Ga (Ea a)) \<or> \<not> b = put\<^bsub>va\<^esub> a (Fa (Ea a) \<or> \<not> Fa (Ea a) \<and> Ga (Ea a)) \<and> (\<not> Fa (Ea a) \<or> \<not> b = put\<^bsub>va\<^esub> a (Fa (Ea a)))"
+    by presburger
+  then have "\<not> ((\<not> Fa (Ea a) \<or> \<not> b = put\<^bsub>va\<^esub> a (Fa (Ea a))) \<and> (Fa (Ea a) \<or> \<not> b = put\<^bsub>va\<^esub> a (Ga (Ea a)))) = (b = put\<^bsub>va\<^esub> a (Fa (Ea a) \<or> \<not> Fa (Ea a) \<and> Ga (Ea a)))"
+    by fastforce
+  then show "(Fa (Ea a) \<and> b = put\<^bsub>va\<^esub> a (Fa (Ea a)) \<or> \<not> Fa (Ea a) \<and> b = put\<^bsub>va\<^esub> a (Ga (Ea a))) = (b = put\<^bsub>va\<^esub> a (Fa (Ea a) \<or> \<not> Fa (Ea a) \<and> Ga (Ea a)))"
+    by meson
+qed 
 
 lemma assign_cond_If_bop5[symbolic_exec_assign_bop]:
   assumes 1: "mwb_lens v" and 2:"v \<sharp> exp1" and 3:"v \<sharp> exp2"
@@ -313,7 +347,15 @@ lemma assign_cond_If_bop5[symbolic_exec_assign_bop]:
           (v:== (bop F exp1 (&v))) \<triangleleft>bop F exp1 (&v)\<triangleright>\<^sub>r (v:== (bop G (&v) exp2))) =
          (v:== (trop If (bop F exp1 E) (bop F exp1 E) (bop G E exp2)))" 
   using 1 2 3
-  by rel_auto
+proof (rel_simp, transfer)
+  fix a :: 'a and b :: 'a and va :: "bool \<Longrightarrow> 'a" and Fa :: "bool \<Rightarrow> bool" and Ea :: "'a \<Rightarrow> bool" and Ga :: "bool \<Rightarrow> bool"
+  have "Fa (Ea a) \<longrightarrow> (Fa (Ea a) \<and> b = put\<^bsub>va\<^esub> a (Fa (Ea a)) \<or> \<not> Fa (Ea a) \<and> b = put\<^bsub>va\<^esub> a (Ga (Ea a))) \<and> b = put\<^bsub>va\<^esub> a (Fa (Ea a) \<or> \<not> Fa (Ea a) \<and> Ga (Ea a)) \<or> \<not> b = put\<^bsub>va\<^esub> a (Fa (Ea a) \<or> \<not> Fa (Ea a) \<and> Ga (Ea a)) \<and> (\<not> Fa (Ea a) \<or> \<not> b = put\<^bsub>va\<^esub> a (Fa (Ea a)))"
+    by presburger
+  then have "\<not> ((\<not> Fa (Ea a) \<or> \<not> b = put\<^bsub>va\<^esub> a (Fa (Ea a))) \<and> (Fa (Ea a) \<or> \<not> b = put\<^bsub>va\<^esub> a (Ga (Ea a)))) = (b = put\<^bsub>va\<^esub> a (Fa (Ea a) \<or> \<not> Fa (Ea a) \<and> Ga (Ea a)))"
+    by fastforce
+  then show "(Fa (Ea a) \<and> b = put\<^bsub>va\<^esub> a (Fa (Ea a)) \<or> \<not> Fa (Ea a) \<and> b = put\<^bsub>va\<^esub> a (Ga (Ea a))) = (b = put\<^bsub>va\<^esub> a (Fa (Ea a) \<or> \<not> Fa (Ea a) \<and> Ga (Ea a)))"
+    by meson
+qed 
 
 lemma assign_cond_If_bop6[symbolic_exec_assign_bop]:
   assumes 1: "mwb_lens v" and 2:"v \<sharp> exp1" and 3:"v \<sharp> exp2"
@@ -321,7 +363,15 @@ lemma assign_cond_If_bop6[symbolic_exec_assign_bop]:
           (v:== (bop F exp1 (&v))) \<triangleleft>bop F exp1 (&v)\<triangleright>\<^sub>r (v:== (bop G exp2 (&v)))) =
          (v:== (trop If (bop F exp1 E) (bop F exp1 E) (bop G exp2 E)))" 
   using 1 2 3
-  by rel_auto
+proof (rel_simp, transfer)
+  fix a :: 'a and b :: 'a and va :: "bool \<Longrightarrow> 'a" and Fa :: "bool \<Rightarrow> bool" and Ea :: "'a \<Rightarrow> bool" and Ga :: "bool \<Rightarrow> bool"
+  have "Fa (Ea a) \<longrightarrow> (Fa (Ea a) \<and> b = put\<^bsub>va\<^esub> a (Fa (Ea a)) \<or> \<not> Fa (Ea a) \<and> b = put\<^bsub>va\<^esub> a (Ga (Ea a))) \<and> b = put\<^bsub>va\<^esub> a (Fa (Ea a) \<or> \<not> Fa (Ea a) \<and> Ga (Ea a)) \<or> \<not> b = put\<^bsub>va\<^esub> a (Fa (Ea a) \<or> \<not> Fa (Ea a) \<and> Ga (Ea a)) \<and> (\<not> Fa (Ea a) \<or> \<not> b = put\<^bsub>va\<^esub> a (Fa (Ea a)))"
+    by presburger
+  then have "\<not> ((\<not> Fa (Ea a) \<or> \<not> b = put\<^bsub>va\<^esub> a (Fa (Ea a))) \<and> (Fa (Ea a) \<or> \<not> b = put\<^bsub>va\<^esub> a (Ga (Ea a)))) = (b = put\<^bsub>va\<^esub> a (Fa (Ea a) \<or> \<not> Fa (Ea a) \<and> Ga (Ea a)))"
+    by fastforce
+  then show "(Fa (Ea a) \<and> b = put\<^bsub>va\<^esub> a (Fa (Ea a)) \<or> \<not> Fa (Ea a) \<and> b = put\<^bsub>va\<^esub> a (Ga (Ea a))) = (b = put\<^bsub>va\<^esub> a (Fa (Ea a) \<or> \<not> Fa (Ea a) \<and> Ga (Ea a)))"
+    by meson
+qed 
 
 lemma assign_cond_If_trop[symbolic_exec_assign_trop]:
   assumes 1: "mwb_lens v" and 2:"v \<sharp> exp1" and 3:"v \<sharp> exp2"
@@ -329,7 +379,15 @@ lemma assign_cond_If_trop[symbolic_exec_assign_trop]:
          (v:== (trop F exp1 exp2 (&v))) \<triangleleft>trop F exp1 exp2 (&v)\<triangleright>\<^sub>r (v:== (trop G exp1 exp2 (&v)))) =
          (v:== (trop If (trop F exp1 exp2 E) (trop F exp1 exp2 E) (trop G exp1 exp2 E)))" 
   using 1 2 3
-  by rel_auto
+proof (rel_simp, transfer)
+  fix a :: 'a and b :: 'a and va :: "bool \<Longrightarrow> 'a" and Fa :: "bool \<Rightarrow> bool" and Ea :: "'a \<Rightarrow> bool" and Ga :: "bool \<Rightarrow> bool"
+  have "Fa (Ea a) \<longrightarrow> (Fa (Ea a) \<and> b = put\<^bsub>va\<^esub> a (Fa (Ea a)) \<or> \<not> Fa (Ea a) \<and> b = put\<^bsub>va\<^esub> a (Ga (Ea a))) \<and> b = put\<^bsub>va\<^esub> a (Fa (Ea a) \<or> \<not> Fa (Ea a) \<and> Ga (Ea a)) \<or> \<not> b = put\<^bsub>va\<^esub> a (Fa (Ea a) \<or> \<not> Fa (Ea a) \<and> Ga (Ea a)) \<and> (\<not> Fa (Ea a) \<or> \<not> b = put\<^bsub>va\<^esub> a (Fa (Ea a)))"
+    by presburger
+  then have "\<not> ((\<not> Fa (Ea a) \<or> \<not> b = put\<^bsub>va\<^esub> a (Fa (Ea a))) \<and> (Fa (Ea a) \<or> \<not> b = put\<^bsub>va\<^esub> a (Ga (Ea a)))) = (b = put\<^bsub>va\<^esub> a (Fa (Ea a) \<or> \<not> Fa (Ea a) \<and> Ga (Ea a)))"
+    by fastforce
+  then show "(Fa (Ea a) \<and> b = put\<^bsub>va\<^esub> a (Fa (Ea a)) \<or> \<not> Fa (Ea a) \<and> b = put\<^bsub>va\<^esub> a (Ga (Ea a))) = (b = put\<^bsub>va\<^esub> a (Fa (Ea a) \<or> \<not> Fa (Ea a) \<and> Ga (Ea a)))"
+    by meson
+qed 
 
 lemma assign_cond_If_trop1[symbolic_exec_assign_trop]:
   assumes 1: "mwb_lens v" and 2:"v \<sharp> exp1" and 3:"v \<sharp> exp2"
@@ -337,7 +395,15 @@ lemma assign_cond_If_trop1[symbolic_exec_assign_trop]:
           (v:== (trop F exp1 (&v) exp2)) \<triangleleft>trop F exp1 (&v) exp2\<triangleright>\<^sub>r (v:== (trop G exp1 (&v) exp2))) =
          (v:== (trop If (trop F exp1 E exp2) (trop F exp1 E exp2) (trop G exp1 E exp2)))" 
   using 1 2 3
-  by rel_auto
+proof (rel_simp, transfer)
+  fix a :: 'a and b :: 'a and va :: "bool \<Longrightarrow> 'a" and Fa :: "bool \<Rightarrow> bool" and Ea :: "'a \<Rightarrow> bool" and Ga :: "bool \<Rightarrow> bool"
+  have "Fa (Ea a) \<longrightarrow> (Fa (Ea a) \<and> b = put\<^bsub>va\<^esub> a (Fa (Ea a)) \<or> \<not> Fa (Ea a) \<and> b = put\<^bsub>va\<^esub> a (Ga (Ea a))) \<and> b = put\<^bsub>va\<^esub> a (Fa (Ea a) \<or> \<not> Fa (Ea a) \<and> Ga (Ea a)) \<or> \<not> b = put\<^bsub>va\<^esub> a (Fa (Ea a) \<or> \<not> Fa (Ea a) \<and> Ga (Ea a)) \<and> (\<not> Fa (Ea a) \<or> \<not> b = put\<^bsub>va\<^esub> a (Fa (Ea a)))"
+    by presburger
+  then have "\<not> ((\<not> Fa (Ea a) \<or> \<not> b = put\<^bsub>va\<^esub> a (Fa (Ea a))) \<and> (Fa (Ea a) \<or> \<not> b = put\<^bsub>va\<^esub> a (Ga (Ea a)))) = (b = put\<^bsub>va\<^esub> a (Fa (Ea a) \<or> \<not> Fa (Ea a) \<and> Ga (Ea a)))"
+    by fastforce
+  then show "(Fa (Ea a) \<and> b = put\<^bsub>va\<^esub> a (Fa (Ea a)) \<or> \<not> Fa (Ea a) \<and> b = put\<^bsub>va\<^esub> a (Ga (Ea a))) = (b = put\<^bsub>va\<^esub> a (Fa (Ea a) \<or> \<not> Fa (Ea a) \<and> Ga (Ea a)))"
+    by meson
+qed 
 
 lemma assign_cond_If_trop2[symbolic_exec_assign_trop]:
   assumes 1: "mwb_lens v" and 2:"v \<sharp> exp1" and 3:"v \<sharp> exp2"
@@ -345,7 +411,15 @@ lemma assign_cond_If_trop2[symbolic_exec_assign_trop]:
           (v:== (trop F (&v) exp1 exp2)) \<triangleleft>trop F (&v) exp1 exp2\<triangleright>\<^sub>r (v:== (trop G (&v) exp1 exp2))) =
          (v:== (trop If (trop F E exp1 exp2) (trop F E exp1 exp2) (trop G E exp1 exp2)))" 
   using 1 2 3
-  by rel_auto
+proof (rel_simp, transfer)
+  fix a :: 'a and b :: 'a and va :: "bool \<Longrightarrow> 'a" and Fa :: "bool \<Rightarrow> bool" and Ea :: "'a \<Rightarrow> bool" and Ga :: "bool \<Rightarrow> bool"
+  have "Fa (Ea a) \<longrightarrow> (Fa (Ea a) \<and> b = put\<^bsub>va\<^esub> a (Fa (Ea a)) \<or> \<not> Fa (Ea a) \<and> b = put\<^bsub>va\<^esub> a (Ga (Ea a))) \<and> b = put\<^bsub>va\<^esub> a (Fa (Ea a) \<or> \<not> Fa (Ea a) \<and> Ga (Ea a)) \<or> \<not> b = put\<^bsub>va\<^esub> a (Fa (Ea a) \<or> \<not> Fa (Ea a) \<and> Ga (Ea a)) \<and> (\<not> Fa (Ea a) \<or> \<not> b = put\<^bsub>va\<^esub> a (Fa (Ea a)))"
+    by presburger
+  then have "\<not> ((\<not> Fa (Ea a) \<or> \<not> b = put\<^bsub>va\<^esub> a (Fa (Ea a))) \<and> (Fa (Ea a) \<or> \<not> b = put\<^bsub>va\<^esub> a (Ga (Ea a)))) = (b = put\<^bsub>va\<^esub> a (Fa (Ea a) \<or> \<not> Fa (Ea a) \<and> Ga (Ea a)))"
+    by fastforce
+  then show "(Fa (Ea a) \<and> b = put\<^bsub>va\<^esub> a (Fa (Ea a)) \<or> \<not> Fa (Ea a) \<and> b = put\<^bsub>va\<^esub> a (Ga (Ea a))) = (b = put\<^bsub>va\<^esub> a (Fa (Ea a) \<or> \<not> Fa (Ea a) \<and> Ga (Ea a)))"
+    by meson
+qed 
 
 lemma assign_cond_If_trop3[symbolic_exec_assign_trop]:
   assumes 1: "mwb_lens v" and 2:"v \<sharp> exp1" and 3:"v \<sharp> exp2" and 4:"v \<sharp> exp3" and 5:"v \<sharp> exp4"
@@ -353,7 +427,15 @@ lemma assign_cond_If_trop3[symbolic_exec_assign_trop]:
           (v:== (trop F exp1 exp2 (&v))) \<triangleleft>trop F exp1 exp2 (&v)\<triangleright>\<^sub>r (v:== (trop G exp3 exp4 (&v)))) =
          (v:== (trop If (trop F exp1 exp2 E) (trop F exp1 exp2 E) (trop G exp3 exp4 E)))" 
   using 1 2 3 4 5
-  by rel_auto
+proof (rel_simp, transfer)
+  fix a :: 'a and b :: 'a and va :: "bool \<Longrightarrow> 'a" and Fa :: "bool \<Rightarrow> bool" and Ea :: "'a \<Rightarrow> bool" and Ga :: "bool \<Rightarrow> bool"
+  have "Fa (Ea a) \<longrightarrow> (Fa (Ea a) \<and> b = put\<^bsub>va\<^esub> a (Fa (Ea a)) \<or> \<not> Fa (Ea a) \<and> b = put\<^bsub>va\<^esub> a (Ga (Ea a))) \<and> b = put\<^bsub>va\<^esub> a (Fa (Ea a) \<or> \<not> Fa (Ea a) \<and> Ga (Ea a)) \<or> \<not> b = put\<^bsub>va\<^esub> a (Fa (Ea a) \<or> \<not> Fa (Ea a) \<and> Ga (Ea a)) \<and> (\<not> Fa (Ea a) \<or> \<not> b = put\<^bsub>va\<^esub> a (Fa (Ea a)))"
+    by presburger
+  then have "\<not> ((\<not> Fa (Ea a) \<or> \<not> b = put\<^bsub>va\<^esub> a (Fa (Ea a))) \<and> (Fa (Ea a) \<or> \<not> b = put\<^bsub>va\<^esub> a (Ga (Ea a)))) = (b = put\<^bsub>va\<^esub> a (Fa (Ea a) \<or> \<not> Fa (Ea a) \<and> Ga (Ea a)))"
+    by fastforce
+  then show "(Fa (Ea a) \<and> b = put\<^bsub>va\<^esub> a (Fa (Ea a)) \<or> \<not> Fa (Ea a) \<and> b = put\<^bsub>va\<^esub> a (Ga (Ea a))) = (b = put\<^bsub>va\<^esub> a (Fa (Ea a) \<or> \<not> Fa (Ea a) \<and> Ga (Ea a)))"
+    by meson
+qed 
 
 lemma assign_cond_If_trop4[symbolic_exec_assign_trop]:
   assumes 1: "mwb_lens v" and 2:"v \<sharp> exp1" and 3:"v \<sharp> exp2" and 4:"v \<sharp> exp3" and 5:"v \<sharp> exp4"
@@ -361,7 +443,15 @@ lemma assign_cond_If_trop4[symbolic_exec_assign_trop]:
          (v:== (trop F exp1 (&v) exp2)) \<triangleleft>trop F exp1 (&v) exp2\<triangleright>\<^sub>r (v:== (trop G exp3 (&v) exp4))) =
          (v:== (trop If (trop F exp1 E exp2) (trop F exp1 E exp2) (trop G exp3 E exp4)))" 
   using 1 2 3 4 5
-  by rel_auto
+proof (rel_simp, transfer)
+  fix a :: 'a and b :: 'a and va :: "bool \<Longrightarrow> 'a" and Fa :: "bool \<Rightarrow> bool" and Ea :: "'a \<Rightarrow> bool" and Ga :: "bool \<Rightarrow> bool"
+  have "Fa (Ea a) \<longrightarrow> (Fa (Ea a) \<and> b = put\<^bsub>va\<^esub> a (Fa (Ea a)) \<or> \<not> Fa (Ea a) \<and> b = put\<^bsub>va\<^esub> a (Ga (Ea a))) \<and> b = put\<^bsub>va\<^esub> a (Fa (Ea a) \<or> \<not> Fa (Ea a) \<and> Ga (Ea a)) \<or> \<not> b = put\<^bsub>va\<^esub> a (Fa (Ea a) \<or> \<not> Fa (Ea a) \<and> Ga (Ea a)) \<and> (\<not> Fa (Ea a) \<or> \<not> b = put\<^bsub>va\<^esub> a (Fa (Ea a)))"
+    by presburger
+  then have "\<not> ((\<not> Fa (Ea a) \<or> \<not> b = put\<^bsub>va\<^esub> a (Fa (Ea a))) \<and> (Fa (Ea a) \<or> \<not> b = put\<^bsub>va\<^esub> a (Ga (Ea a)))) = (b = put\<^bsub>va\<^esub> a (Fa (Ea a) \<or> \<not> Fa (Ea a) \<and> Ga (Ea a)))"
+    by fastforce
+  then show "(Fa (Ea a) \<and> b = put\<^bsub>va\<^esub> a (Fa (Ea a)) \<or> \<not> Fa (Ea a) \<and> b = put\<^bsub>va\<^esub> a (Ga (Ea a))) = (b = put\<^bsub>va\<^esub> a (Fa (Ea a) \<or> \<not> Fa (Ea a) \<and> Ga (Ea a)))"
+    by meson
+qed 
 
 lemma assign_cond_If_trop5[symbolic_exec_assign_trop]:
   assumes 1: "mwb_lens v" and 2:"v \<sharp> exp1" and 3:"v \<sharp> exp2" and 4:"v \<sharp> exp3" and 5:"v \<sharp> exp4"
@@ -369,99 +459,94 @@ lemma assign_cond_If_trop5[symbolic_exec_assign_trop]:
           (v:== (trop F (&v) exp1 exp2)) \<triangleleft>trop F (&v) exp1 exp2\<triangleright>\<^sub>r (v:== (trop G (&v) exp3 exp4))) =
          (v:== (trop If (trop F E exp1 exp2) (trop F E exp1 exp2) (trop G E exp3 exp4)))" 
   using 1 2 3 4 5
-  by rel_auto
+proof (rel_simp, transfer)
+  fix a :: 'a and b :: 'a and va :: "bool \<Longrightarrow> 'a" and Fa :: "bool \<Rightarrow> bool" and Ea :: "'a \<Rightarrow> bool" and Ga :: "bool \<Rightarrow> bool"
+  have "Fa (Ea a) \<longrightarrow> (Fa (Ea a) \<and> b = put\<^bsub>va\<^esub> a (Fa (Ea a)) \<or> \<not> Fa (Ea a) \<and> b = put\<^bsub>va\<^esub> a (Ga (Ea a))) \<and> b = put\<^bsub>va\<^esub> a (Fa (Ea a) \<or> \<not> Fa (Ea a) \<and> Ga (Ea a)) \<or> \<not> b = put\<^bsub>va\<^esub> a (Fa (Ea a) \<or> \<not> Fa (Ea a) \<and> Ga (Ea a)) \<and> (\<not> Fa (Ea a) \<or> \<not> b = put\<^bsub>va\<^esub> a (Fa (Ea a)))"
+    by presburger
+  then have "\<not> ((\<not> Fa (Ea a) \<or> \<not> b = put\<^bsub>va\<^esub> a (Fa (Ea a))) \<and> (Fa (Ea a) \<or> \<not> b = put\<^bsub>va\<^esub> a (Ga (Ea a)))) = (b = put\<^bsub>va\<^esub> a (Fa (Ea a) \<or> \<not> Fa (Ea a) \<and> Ga (Ea a)))"
+    by fastforce
+  then show "(Fa (Ea a) \<and> b = put\<^bsub>va\<^esub> a (Fa (Ea a)) \<or> \<not> Fa (Ea a) \<and> b = put\<^bsub>va\<^esub> a (Ga (Ea a))) = (b = put\<^bsub>va\<^esub> a (Fa (Ea a) \<or> \<not> Fa (Ea a) \<and> Ga (Ea a)))"
+    by meson
+qed 
 
 subsection {*Conditional Laws*}
 text{*In this section we introduce the algebraic laws of programming related to the conditional
       statement.*}
 
 lemma cond_idem[symbolic_exec]:
-  "(IF b THEN P ELSE P) = P" 
+  "(P \<triangleleft> b \<triangleright> P) = P" 
   by rel_auto
 
 lemma cond_symm:
-  "(IF b THEN P ELSE Q) = (IF \<not> b THEN Q ELSE P)" 
+  "(P \<triangleleft> b \<triangleright> Q) = (Q \<triangleleft>\<not> b\<triangleright> P)" 
   by rel_auto
 
 lemma cond_assoc: 
-  "(IF b THEN P ELSE (IF b THEN Q ELSE R)) =  
-   (IF b THEN (IF b THEN P ELSE Q) ELSE R)"  
-   by rel_auto
+  "(P \<triangleleft> b \<triangleright> (Q \<triangleleft> b \<triangleright> R)) = ((P \<triangleleft> b \<triangleright> Q) \<triangleleft> b \<triangleright>  R)"  
+  by rel_auto
 
 lemma cond_distr[symbolic_exec]: 
-  "(IF b THEN (IF b' THEN P ELSE R) ELSE (IF b' THEN Q ELSE R))=  
-   (IF b' THEN (IF b THEN P ELSE Q) ELSE R)" 
+  "((P \<triangleleft> b'\<triangleright> R) \<triangleleft> b \<triangleright> (Q \<triangleleft> b'\<triangleright> R))= ((P \<triangleleft> b \<triangleright> Q) \<triangleleft> b'\<triangleright> R)" 
   by rel_auto
 
-lemma cond_unit_T [simp, symbolic_exec_ex]:"(IF true THEN P ELSE Q) = P" 
-  by rel_auto
+lemma cond_unit_T [symbolic_exec_ex]:
+  "(P \<triangleleft>true\<triangleright> Q) = P" 
+  by auto
 
-lemma cond_unit_F [simp, symbolic_exec_ex]:"(IF false THEN P ELSE Q) = Q" 
-  by rel_auto
+lemma cond_unit_F [symbolic_exec_ex]:
+  "(P \<triangleleft>false\<triangleright> Q) = Q" 
+  by auto
 
 lemma cond_and_T_integrate[symbolic_exec]:
-  "((P \<and> b) \<or> (IF b THEN Q ELSE R)) = (IF b THEN (P \<or> Q) ELSE R)"
+  "((P \<and> b) \<or> (Q \<triangleleft> b \<triangleright> R)) = ((P \<or> Q) \<triangleleft> b \<triangleright> R)"
   by rel_auto
 
 lemma cond_L6[symbolic_exec]: 
-  "(IF b THEN P ELSE (IF b THEN Q ELSE R)) = 
-   (IF b THEN P ELSE R)" 
+  "(P \<triangleleft> b \<triangleright> (Q \<triangleleft> b \<triangleright> R)) = (P \<triangleleft> b \<triangleright> R)" 
   by rel_auto
 
 lemma cond_L7[symbolic_exec]: 
-  "(IF b THEN P ELSE (IF c THEN P ELSE Q)) = 
-   (IF b \<or> c THEN P ELSE Q)"
+  "(P \<triangleleft> b \<triangleright> (P \<triangleleft> c \<triangleright> Q)) = (P \<triangleleft> b \<or> c \<triangleright> Q)"
   by rel_auto
 
 lemma cond_and_distr[symbolic_exec]: 
-  "(IF b THEN (P \<and> Q) ELSE (R \<and> S)) = 
-   ((IF b THEN P ELSE R) \<and> (IF b THEN Q ELSE S))"  
+  "((P \<and> Q) \<triangleleft> b \<triangleright> (R \<and> S)) = ((P \<triangleleft> b \<triangleright> R) \<and> (Q \<triangleleft> b \<triangleright> S))"  
   by rel_auto
 
 lemma cond_or_distr[symbolic_exec]: 
-  "(IF b THEN (P \<or> Q) ELSE (R \<or> S)) = 
-   ((IF b THEN P ELSE R) \<or> (IF b THEN Q ELSE S))" 
+  "((P \<or> Q) \<triangleleft> b \<triangleright> (R \<or> S)) = ((P \<triangleleft> b \<triangleright> R) \<or> (Q \<triangleleft> b \<triangleright> S))" 
   by rel_auto
 
 lemma cond_imp_distr[symbolic_exec]:
-  "(IF b THEN (P \<Rightarrow> Q) ELSE (R \<Rightarrow> S)) = 
-   ((IF b THEN P ELSE R) \<Rightarrow> (IF b THEN Q ELSE S))" 
+  "((P \<Rightarrow> Q) \<triangleleft> b \<triangleright> (R \<Rightarrow> S)) = 
+   ((P \<triangleleft> b \<triangleright> R) \<Rightarrow> (Q \<triangleleft> b \<triangleright> S))" 
   by rel_auto
 
 lemma cond_eq_distr[symbolic_exec]:
-  "(IF b THEN (P \<Leftrightarrow> Q) ELSE (R \<Leftrightarrow> S)) = 
-   ((IF b THEN P ELSE R) \<Leftrightarrow> (IF b THEN Q ELSE S))"
+  "((P \<Leftrightarrow> Q) \<triangleleft> b \<triangleright> (R \<Leftrightarrow> S)) = 
+   ((P \<triangleleft> b \<triangleright> R) \<Leftrightarrow> (Q \<triangleleft> b \<triangleright> S))"
   by rel_auto
 
 lemma cond_conj_distr[symbolic_exec]:
-  "(P \<and> (IF b THEN Q ELSE S)) = (IF b THEN (P \<and> Q) ELSE (P \<and> S))"  
+  "(P \<and> (Q \<triangleleft> b \<triangleright> S)) = ((P \<and> Q) \<triangleleft> b \<triangleright> (P \<and> S))"  
   by rel_auto
 
 lemma cond_disj_distr [symbolic_exec]:
-  "(P \<or> (IF b THEN Q ELSE S)) = (IF b THEN (P \<or> Q) ELSE (P \<or> S))" 
+  "(P \<or> (Q \<triangleleft> b \<triangleright> S)) = ((P \<or> Q) \<triangleleft> b \<triangleright> (P \<or> S))" 
   by rel_auto 
 
 lemma cond_neg[symbolic_exec]: 
-  "\<not> (IF b THEN P ELSE Q) = (IF b THEN (\<not> P) ELSE (\<not> Q))"
+  "\<not> (P \<triangleleft> b \<triangleright> Q) = ((\<not> P) \<triangleleft> b \<triangleright> (\<not> Q))"
   by rel_auto 
-
-(*lemma cond_USUP_dist: 
-  "IF b THEN (\<Squnion> P\<in>S \<bullet> F(P)) ELSE (\<Squnion> P\<in>S \<bullet> G(P)) = (IF b THEN \<Squnion> P\<in>S \<bullet> F(P) ELSE G(P))"
-  by (subst uexpr_eq_iff, auto simp add: disj_upred_def conj_upred_def not_upred_def cond_def UINF.rep_eq uminus_uexpr_def inf_uexpr.rep_eq sup_uexpr.rep_eq uop.rep_eq bop.rep_eq lit.rep_eq)
-
-lemma cond_UINF_dist: "(\<Sqinter> P\<in>S \<bullet> F(P)) \<triangleleft> b \<triangleright> (\<Sqinter> P\<in>S \<bullet> G(P)) = (\<Sqinter> P\<in>S \<bullet> F(P) \<triangleleft> b \<triangleright> G(P))"
-  by (subst uexpr_eq_iff, auto simp add: disj_upred_def conj_upred_def not_upred_def cond_def USUP.rep_eq uminus_uexpr_def inf_uexpr.rep_eq sup_uexpr.rep_eq uop.rep_eq bop.rep_eq lit.rep_eq)
-*)
 
 lemma cond_conj[symbolic_exec]: 
-  "(IF b \<and> c THEN P ELSE Q) = IF b THEN (IF c THEN P ELSE Q) ELSE Q"
+  "(P \<triangleleft>b \<and> c\<triangleright> Q) = (P \<triangleleft> c \<triangleright> Q) \<triangleleft> b \<triangleright> Q"
   by rel_auto 
     
-
 (*IF Theorem by Hoare: It optimize nested IF*)
 theorem COND12[symbolic_exec]: 
-  "(IF bexp1 THEN (IF bexp2 THEN C1 ELSE C3) ELSE (IF bexp3 THEN C2 ELSE C3)) =
-   (IF (trop If bexp1 bexp2 bexp3) THEN (IF bexp1 THEN C1 ELSE C2) ELSE C3)"
+  "((C1 \<triangleleft>bexp2\<triangleright> C3) \<triangleleft>bexp1\<triangleright> (C2 \<triangleleft>bexp3\<triangleright> C3)) =
+   ((C1 \<triangleleft>bexp1\<triangleright> C2) \<triangleleft>(bexp2 \<triangleleft>bexp1\<triangleright>bexp3)\<triangleright> C3)"
   by rel_auto 
  
 lemma comp_cond_left_distr:
@@ -470,27 +555,28 @@ lemma comp_cond_left_distr:
  
 lemma cond_var_subst_left:
   assumes "vwb_lens x"
-  shows "(IF &x THEN P\<lbrakk>true/x\<rbrakk> ELSE Q) = (IF  &x THEN P ELSE Q)"
+  shows "(P\<lbrakk>true/x\<rbrakk> \<triangleleft>&x \<triangleright> Q) = (P \<triangleleft>&x \<triangleright> Q)"
   using assms
-  by (metis cond_def conj_var_subst pr_var_def upred_eq_true utp_pred.inf.commute)
+  apply rel_auto apply transfer
+  using vwb_lens.put_eq by fastforce 
 
 lemma cond_var_subst_right:
   assumes "vwb_lens x"
-  shows "(IF &x THEN P ELSE Q\<lbrakk>false/x\<rbrakk>) = (IF &x THEN P ELSE Q)"
+  shows "(P \<triangleleft>&x \<triangleright> Q\<lbrakk>false/x\<rbrakk>) = (P \<triangleleft>&x \<triangleright> Q)"
   using assms
-  by (metis cond_def  conj_var_subst pr_var_def upred_eq_false utp_pred.inf.commute)
-
+  apply rel_auto apply transfer
+  by (metis (full_types) vwb_lens.put_eq)
 
 lemma cond_var_split:
-  "vwb_lens x \<Longrightarrow> (IF &x THEN P\<lbrakk>true/x\<rbrakk> ELSE P\<lbrakk>false/x\<rbrakk>) = P"
+  "vwb_lens x \<Longrightarrow> (P\<lbrakk>true/x\<rbrakk> \<triangleleft>&x \<triangleright> P\<lbrakk>false/x\<rbrakk>) = P"
   by (rel_auto, (metis (full_types) vwb_lens.put_eq)+)
 
 lemma cond_seq_left_distr:
-  "out\<alpha> \<sharp> b \<Longrightarrow> ((IF b THEN P ELSE Q) ;; R) = (IF b THEN (P ;; R) ELSE (Q ;; R))"
+  "out\<alpha> \<sharp> b \<Longrightarrow> ((P \<triangleleft> b \<triangleright> Q) ;; R) = ((P ;; R) \<triangleleft> b \<triangleright> (Q ;; R))"
   by rel_auto
 
 lemma cond_seq_right_distr:
-  "in\<alpha> \<sharp> b \<Longrightarrow> (P ;; (IF b THEN Q ELSE R)) = (IF b THEN (P ;; Q) ELSE (P ;; R))"
+  "in\<alpha> \<sharp> b \<Longrightarrow> (P ;; (Q \<triangleleft> b \<triangleright> R)) = ((P ;; Q) \<triangleleft> b \<triangleright> (P ;; R))"
   by rel_auto
 
 subsection {*Sequential Laws*}
@@ -533,7 +619,7 @@ lemma seqr_middle:
   assumes "vwb_lens x"
   shows "(P ;; Q) = (\<^bold>\<exists> v \<bullet> P\<lbrakk>\<guillemotleft>v\<guillemotright>/$x\<acute>\<rbrakk> ;; Q\<lbrakk>\<guillemotleft>v\<guillemotright>/$x\<rbrakk>)"
   using assms
-  apply (rel_auto)
+  apply (rel_auto robust)
   apply (rename_tac xa P Q a b y)
   apply (rule_tac x="get\<^bsub>xa\<^esub> y" in exI)
   apply (rule_tac x="y" in exI)
@@ -570,7 +656,7 @@ lemma seq_var_ident_lift:
   using assms
   by (rel_auto, metis (no_types, lifting) vwb_lens_wb wb_lens_weak weak_lens.put_get)
 
-lemma seqr_skip: "SKIP ;; C = C ;; SKIP"
+lemma seqr_skip: "II ;; C = C ;; II"
   by (metis seqr_left_unit seqr_right_unit)
 
 (*The rules SEQ6 SEQ7 related to SEQ and non-deterministic choice are missing for now*)
@@ -580,45 +666,71 @@ text{*In this section we introduce the algebraic laws of programming related to 
       statement.*}
 
 theorem while_unfold:
-  "WHILE b DO P OD = ((P ;; WHILE b DO P OD) \<triangleleft> b \<triangleright>\<^sub>r SKIP)"
+  "while b do P od = ((P ;; while b do P od) \<triangleleft> b \<triangleright>\<^sub>r II)"
 proof -
-  have m:"mono (\<lambda>X. (P ;; X) \<triangleleft> b \<triangleright>\<^sub>r SKIP)"
+  have m:"mono (\<lambda>X. (P ;; X) \<triangleleft> b \<triangleright>\<^sub>r II)"
     by (auto intro: monoI seqr_mono cond_mono)
-  have "(WHILE b DO P OD) = (\<nu> X \<bullet> (P ;; X) \<triangleleft> b \<triangleright>\<^sub>r SKIP)"
-    by (simp add: While_def)
-  also have "... = ((P ;; (\<nu> X \<bullet> (P ;; X) \<triangleleft> b \<triangleright>\<^sub>r SKIP)) \<triangleleft> b \<triangleright>\<^sub>r SKIP)"
+  have "(while b do P od) = (\<nu> X \<bullet> (P ;; X) \<triangleleft> b \<triangleright>\<^sub>r II)"
+    by (simp add: while_def)
+  also have "... = ((P ;; (\<nu> X \<bullet> (P ;; X) \<triangleleft> b \<triangleright>\<^sub>r II)) \<triangleleft> b \<triangleright>\<^sub>r II)"
     by (subst lfp_unfold, simp_all add: m)
-  also have "... = ((P ;; WHILE b DO P OD) \<triangleleft> b \<triangleright>\<^sub>r SKIP)"
-    by (simp add: While_def)
+  also have "... = ((P ;; while b do P od) \<triangleleft> b \<triangleright>\<^sub>r II)"
+    by (simp add: while_def)
   finally show ?thesis .
 qed
 
 lemma while_true:
-  assumes 1:"b = true"
-  shows "(WHILE b DO P OD) = (P ;; WHILE b DO P OD)"
-proof -
-  have "(WHILE b DO P OD) = (P ;; WHILE b DO P OD) \<triangleleft> b \<triangleright>\<^sub>r SKIP" 
-    using while_unfold[of b P] by simp
-  also have "... = (P ;; WHILE b DO P OD)" 
-    using 1 by (simp add: aext_true)
-  finally show ?thesis .
-qed
+  shows "(while true do P od) = false"
+  apply (simp add: while_def alpha)
+  apply (rule antisym)
+  apply (simp_all)
+  apply (rule lfp_lowerbound)
+  apply (simp)
+done
 
 lemma while_false:
-  assumes 1:"b = false"
-  shows "(WHILE b DO P OD) = SKIP"
+  shows "(while false do P od) = II"
 proof -
-  have "(WHILE b DO P OD) = (P ;; WHILE b DO P OD) \<triangleleft> b \<triangleright>\<^sub>r SKIP" 
-    using while_unfold[of b P] by simp
-  also have "... = SKIP" 
-    using 1 by (simp add: aext_false)
+  have "(while false do P od) = (P ;; while false do P od) \<triangleleft> false \<triangleright>\<^sub>r II" 
+    using while_unfold[of _ P] by simp
+  also have "... = II" by (simp add: aext_false)
   finally show ?thesis . 
 qed
 
 lemma while_inv_unfold:
-  "while b invr p do P od = ((P ;; while b invr p do P od) \<triangleleft> b \<triangleright>\<^sub>r SKIP)"
+  "while b invr p do P od = ((P ;; while b invr p do P od) \<triangleleft> b \<triangleright>\<^sub>r II)"
   unfolding while_inv_def using while_unfold
   by auto
+
+theorem while_bot_unfold:
+  "while\<^sub>\<bottom> b do P od = ((P ;; while\<^sub>\<bottom> b do P od) \<triangleleft> b \<triangleright>\<^sub>r II)"
+proof -
+  have m:"mono (\<lambda>X. (P ;; X) \<triangleleft> b \<triangleright>\<^sub>r II)"
+    by (auto intro: monoI seqr_mono cond_mono)
+  have "(while\<^sub>\<bottom> b do P od) = (\<mu> X \<bullet> (P ;; X) \<triangleleft> b \<triangleright>\<^sub>r II)"
+    by (simp add: while_bot_def)
+  also have "... = ((P ;; (\<mu> X \<bullet> (P ;; X) \<triangleleft> b \<triangleright>\<^sub>r II)) \<triangleleft> b \<triangleright>\<^sub>r II)"
+    by (subst gfp_unfold, simp_all add: m)
+  also have "... = ((P ;; while\<^sub>\<bottom> b do P od) \<triangleleft> b \<triangleright>\<^sub>r II)"
+    by (simp add: while_bot_def)
+  finally show ?thesis .
+qed
+
+theorem while_bot_false: "while\<^sub>\<bottom> false do P od = II"
+  by (simp add: while_bot_def mu_const alpha)
+
+theorem while_bot_true: "while\<^sub>\<bottom> true do P od = (\<mu> X \<bullet> P ;; X)"
+  by (simp add: while_bot_def alpha)
+
+text {* An infinite loop with a feasible body corresponds to a program error (non-termination). *}
+
+theorem while_infinite: "P ;; true\<^sub>h = true \<Longrightarrow> while\<^sub>\<bottom> true do P od = true"
+  apply (simp add: while_bot_true)
+  apply (rule antisym)
+  apply (simp)
+  apply (rule gfp_upperbound)
+  apply (simp)
+done
 
 subsection {*assume and assert laws*}
 
@@ -628,44 +740,47 @@ lemma assume_twice: "(b\<^sup>\<top> ;; c\<^sup>\<top>) = (b \<and> c)\<^sup>\<t
 lemma assert_twice: "(b\<^sub>\<bottom> ;; c\<^sub>\<bottom>) = (b \<and> c)\<^sub>\<bottom>" 
   by rel_auto
 
+subsection {* Relation algebra laws *}
+
+theorem RA1: "(P ;; (Q ;; R)) = ((P ;; Q) ;; R)"
+  using seqr_assoc by auto
+
+theorem RA2: "(P ;; II) = P" "(II ;; P) = P"
+  by simp_all
+
+theorem RA3: "P\<^sup>-\<^sup>- = P"
+  by simp
+
+theorem RA4: "(P ;; Q)\<^sup>- = (Q\<^sup>- ;; P\<^sup>-)"
+  by simp
+
+theorem RA5: "(P \<or> Q)\<^sup>- = (P\<^sup>- \<or> Q\<^sup>-)"
+  by (rel_auto)
+
+theorem RA6: "((P \<or> Q) ;; R) = ((P;;R) \<or> (Q;;R))"
+  using seqr_or_distl by blast
+
+theorem RA7: "((P\<^sup>- ;; (\<not>(P ;; Q))) \<or> (\<not>Q)) = (\<not>Q)"
+  by (rel_auto)
+
+subsection {* Relational alphabet extension *}
+
+lift_definition rel_alpha_ext :: "'\<beta> hrel \<Rightarrow> ('\<beta> \<Longrightarrow> '\<alpha>) \<Rightarrow> '\<alpha> hrel" (infix "\<oplus>\<^sub>R" 65)
+is "\<lambda> P x (b1, b2). P (get\<^bsub>x\<^esub> b1, get\<^bsub>x\<^esub> b2) \<and> (\<forall> b. b1 \<oplus>\<^sub>L b on x = b2 \<oplus>\<^sub>L b on x)" .
+
+lemma rel_alpha_ext_alt_def:
+  assumes "vwb_lens y" "x +\<^sub>L y \<approx>\<^sub>L 1\<^sub>L" "x \<bowtie> y"
+  shows "P \<oplus>\<^sub>R x = (P \<oplus>\<^sub>p (x \<times>\<^sub>L x) \<and> $y\<acute> =\<^sub>u $y)"
+  using assms
+  apply (rel_auto robust, simp_all add: lens_override_def)
+  apply (metis lens_indep_get lens_indep_sym)
+  apply (metis vwb_lens_def wb_lens.get_put wb_lens_def weak_lens.put_get)
+done
+
+
 subsection {*Tactic setup*}
 text {*In this section we will design a tactic that can be used to automate
        the process of program optimization.*}
-
-method rel_simp' =
-  (unfold upred_defs urel_defs)?,
-  transfer',
-  (simp add: fun_eq_iff relcomp_unfold OO_def
-    lens_defs upred_defs Product_Type.split_beta)?,
-  (simp add: lens_interp_laws)?,
-  clarsimp?
-method rel_auto' = rel_simp', auto?
-
-method symbolic_exec_commands =
-  (simp add: symbolic_exec)?,
-  ((subst symbolic_exec symbolic_exec_ex)+)?,
-  (simp add: symbolic_exec_assign_uop)?,
-  ((subst symbolic_exec_assign_uop)+)?,
-  (simp add: symbolic_exec_assign_bop)?,
-  ((subst symbolic_exec_assign_bop)+)?,
-  (simp add: symbolic_exec_assign_trop)?,
-  ((subst symbolic_exec_assign_trop)+)?,
-  (simp add: symbolic_exec_assign_qtop)?,
-  ((subst symbolic_exec_assign_qtop)+)?,
-  transfer'?,
-  rel_auto'?
-
-lemmas symbolic_exec_all =
-  symbolic_exec
-  symbolic_exec_assign_uop
-  symbolic_exec_assign_bop
-  symbolic_exec_assign_trop
-  symbolic_exec_assign_qtop
-
-method symbolic_exec_commands_min =
-  (simp add: symbolic_exec_all)?,
-  ((subst symbolic_exec_all symbolic_exec_ex)+)?,
-  transfer'?,
-  rel_auto?
+(*TODO*)
 
 end
