WP1-Programming-Languages-Semantics/WP11-C-semantics/src/IMP-Lenses/features_test.thy
@@ -1,0 +1,76 @@
+section \<open>Verification Condition Testing\<close>
+
+theory features_test
+  imports "utp/utp_hoare"
+begin
+
+subsection {*Even count*}
+
+lemma even_count:
+   assumes "vwb_lens i" and  "weak_lens a" and  "vwb_lens j"  and  "weak_lens n"and
+           "i \<bowtie> a" and "i \<bowtie> j" and "i \<bowtie> n"  "a \<bowtie> j" and "a \<bowtie> n" and "j \<bowtie> n" 
+   shows 
+   "\<lbrace>&a =\<^sub>u \<guillemotleft>0::int\<guillemotright> \<and> &n =\<^sub>u \<guillemotleft>1::int\<guillemotright>\<rbrace>
+       i:== &a ;; j :== \<guillemotleft>0::int\<guillemotright> ;; 
+       (&a =\<^sub>u \<guillemotleft>0::int\<guillemotright> \<and> &n =\<^sub>u \<guillemotleft>1::int\<guillemotright> \<and> &j =\<^sub>u \<guillemotleft>0::int\<guillemotright> \<and> &i =\<^sub>u &a)\<^sup>\<top>;; 
+     while  &i <\<^sub>u &n 
+       invr  &a =\<^sub>u \<guillemotleft>0::int\<guillemotright> \<and> &n =\<^sub>u \<guillemotleft>1::int\<guillemotright> \<and> &j =\<^sub>u (((&i + 1) - &a) div 2) \<and> &i \<le>\<^sub>u &n \<and>  &i \<ge>\<^sub>u &a
+       do (j :== &j + \<guillemotleft>1\<guillemotright> \<triangleleft> &i mod \<guillemotleft>2\<guillemotright> =\<^sub>u  \<guillemotleft>0::int\<guillemotright>\<triangleright>\<^sub>r II) ;;  i :== &i + \<guillemotleft>1\<guillemotright> od
+     \<lbrace>&j =\<^sub>u \<guillemotleft>1::int\<guillemotright>\<rbrace>\<^sub>u"
+ apply (insert assms)
+ apply (rule seq_hoare_r)
+  prefer 2
+  apply (rule seq_hoare_r [of _ _ true])
+   apply (rule assigns_hoare_r')
+  apply (rule seq_hoare_r)
+   apply (rule assume_hoare_r)
+   apply (rule skip_hoare_r)
+  prefer 2
+  apply (rule while_invr_hoare_r)
+    apply (rule seq_hoare_r)
+     prefer 2
+     apply (rule assigns_hoare_r')
+    apply (rule cond_hoare_r)
+     apply (rule assigns_hoare_r)
+     prefer 6
+     apply (rule assigns_hoare_r)
+     unfolding lens_indep_def
+     apply rel_auto[1]
+    apply rel_auto[1]
+    using mod_pos_pos_trivial apply auto[1]
+   apply rel_auto[1]
+  apply rel_auto[1]
+ apply rel_auto[1]
+ apply rel_auto[1]
+done
+
+subsection {*testing features*}
+
+text {*block_test1 is a scenario. The scenario represent a program where i is name of the variable
+       in the scope of the initial state s. In the scenario, and using the command block,
+       we create a new variable with the same name inside the block ie., inside the new scope. 
+       Now i is a local var for the scope t.
+       In that case we can use a restore function on the state s to set the variable to its
+       previous value ie.,its value in the scope s, and this before we exit the block.*}
+
+lemma   blocks_test1:
+  assumes "weak_lens i"
+  shows "\<lbrace>true\<rbrace>
+          i :== \<guillemotleft>2::int\<guillemotright>;; 
+          block (i :== \<guillemotleft>5\<guillemotright>) (II) (\<lambda> (s, s') (t, t').  i:== \<guillemotleft>\<lbrakk>\<langle>id\<rangle>\<^sub>s i\<rbrakk>\<^sub>e s\<guillemotright>) (\<lambda> (s, s') (t, t').  II) 
+         \<lbrace>&i =\<^sub>u \<guillemotleft>2::int\<guillemotright>\<rbrace>\<^sub>u"
+  using assms by rel_auto
+
+text {*block_test2 is similar to  block_test1 but the var i is a global var.
+       In that case we can use restore function and the state t to set the variable to its
+       latest value, ie.,its value in in the scope t,probably modified inside the scope of the block.*}
+
+lemma   blocks_test2:
+  assumes "weak_lens i"
+  shows "\<lbrace>true\<rbrace>
+          i :== \<guillemotleft>2::int\<guillemotright>;; 
+          block (i :== \<guillemotleft>5\<guillemotright>) (II) (\<lambda> (s, s') (t, t').  i:== \<guillemotleft>\<lbrakk>\<langle>id\<rangle>\<^sub>s i\<rbrakk>\<^sub>e t\<guillemotright>) (\<lambda> (s, s') (t, t').  II) 
+         \<lbrace>&i =\<^sub>u \<guillemotleft>5::int\<guillemotright>\<rbrace>\<^sub>u"
+  using assms by rel_auto
+
+end
